examples/find/find_spec.v
@@ -1,11 +1,11 @@
-(**********************************************************************)
+(* Load Programs. *)(**********************************************************************)
 (*                                                                    *)
 (* FIND, an historical example.                                       *)
 (*                                                                    *)
 (* The proof of this program was originally done by C. A. R. Hoare    *)
 (* and fully detailed in the following paper:                         *)
 (*                                                                    *)
-(* C. A. R. Hoare, "Proof of a Program: FIND", Communications of the  *)
+(* C. A. R. Hoare, , Communications of the  *)
 (* ACM, 14(1), 39--45, January 1971.                                  *)
 (*                                                                    *)
 (**********************************************************************)
@@ -18,42 +18,50 @@ Require Export WhyArrays.
 
 (* parameters = globals of the program *)
 
-Parameter N : Z.   (* size of the array *)
-Parameter f : Z.   (* the `pivot' *)
+Parameter N : Z.
+   (* size of the array *)
+Parameter f : Z.
+   (* the `pivot' *)
 
-Axiom le_1_f : `1 <= f`.
-Axiom le_f_N : `f <= N`.
+Axiom le_1_f : (1 <= f)%Z.
+Axiom le_f_N : (f <= N)%Z.
 
 (* Specification part *)
 
-Definition n_invariant :=
-  [n:Z][A:(array Z)]
-     `f <=n`
-  /\ (p,q:Z)(`1<=p` -> `p<=n` -> `n<q` -> `q<=N` -> (Zle #A[p] #A[q])).
+Definition n_invariant (n:Z) (A:array Z) :=
+  (f <= n)%Z /\
+  (forall p q:Z,
+     (1 <= p)%Z ->
+     (p <= n)%Z ->
+     (n < q)%Z -> (q <= N)%Z -> (access A p <= access A q)%Z).
 
-Definition m_invariant :=
-  [m:Z][A:(array Z)]
-     (Zle m f)
-  /\ (p,q:Z)(`1<=p` -> `p<m` -> `m<=q` -> `q<=N` -> (Zle #A[p] #A[q])).
+Definition m_invariant (m:Z) (A:array Z) :=
+  (m <= f)%Z /\
+  (forall p q:Z,
+     (1 <= p)%Z ->
+     (p < m)%Z ->
+     (m <= q)%Z -> (q <= N)%Z -> (access A p <= access A q)%Z).
 
-Definition i_invariant :=
-  [m,n,i,r:Z][A:(array Z)]
-     (Zle m i)
-  /\ ((p:Z)(`1<=p` -> `p<i` -> (Zle #A[p] r)))
-  /\ (`i<=n` -> (EX p:Z | `i<=p` /\ `p<=n` /\ (Zle r #A[p]))).
+Definition i_invariant (m n i r:Z) (A:array Z) :=
+  (m <= i)%Z /\
+  (forall p:Z, (1 <= p)%Z -> (p < i)%Z -> (access A p <= r)%Z) /\
+  ((i <= n)%Z ->
+    EX p : Z | (i <= p)%Z /\ (p <= n)%Z /\ (r <= access A p)%Z).
   
-Definition j_invariant :=
-  [m,n,j,r:Z][A:(array Z)]
-     (Zle j n)
-  /\ ((q:Z)(`j<q` -> `q<=N` -> (Zle r #A[q])))
-  /\ (`m<=j` -> (EX q:Z | `m<=q` /\ `q<=j` /\ (Zle #A[q] r))).
+Definition j_invariant (m n j r:Z) (A:array Z) :=
+  (j <= n)%Z /\
+  (forall q:Z, (j < q)%Z -> (q <= N)%Z -> (r <= access A q)%Z) /\
+  ((m <= j)%Z ->
+    EX q : Z | (m <= q)%Z /\ (q <= j)%Z /\ (access A q <= r)%Z).
 
-Definition termination :=
-  [i,j,i0,j0,r:Z][A:(array Z)]
-    (`i>i0` /\ `j<j0`) \/ (`i<=f<=j` /\ #A[f]=r).
+Definition termination (i j i0 j0 r:Z) (A:array Z) :=
+  (i > i0)%Z /\ (j < j0)%Z \/ (i <= f <= j)%Z /\ access A f = r.
 
-Definition found :=
-  [A:(array Z)]
-    (p,q:Z)`1<=p` -> `p<=f` -> `f<=q` -> `q<=N` 
-      	     -> (Zle #A[p] #A[f]) /\ (Zle #A[f] #A[q]).
+Definition found (A:array Z) :=
+  forall p q:Z,
+    (1 <= p)%Z ->
+    (p <= f)%Z ->
+    (f <= q)%Z ->
+    (q <= N)%Z ->
+    (access A p <= access A f)%Z /\ (access A f <= access A q)%Z.
 
