examples/heapsort/Inftree.v
@@ -1,4 +1,4 @@
-(**************************************************************************)
+(* Load Programs. *)(**************************************************************************)
 (*                                                                        *)
 (* Proof of the Heapsort Algorithm.                                       *)
 (*                                                                        *)
@@ -7,13 +7,14 @@
 (*                                                                        *)
 (**************************************************************************)
 
-Require ZArith.
-Require Why.
-Require Omega.
+Require Import ZArith.
+Require Import Why.
+Require Import Omega.
 
-Require heap.
+Require Import heap.
 
-Implicit Arguments On.
+Set Implicit Arguments.
+Unset Strict Implicit.
 
 (* We will also need another property about a heap, which is to have
  * all his elements smaller or equal than a given value v.
@@ -22,195 +23,242 @@ Implicit Arguments On.
  * defined as follows:
  *)
 
-Inductive inftree [t:(array Z); n,v:Z] : Z -> Prop :=
-  inftree_cons : (k:Z)
-      `0 <= k <= n` 
-   -> `(access t k) <= v`
-   -> (`2*k+1 <= n` -> (inftree t n v `2*k+1`))
-   -> (`2*k+2 <= n` -> (inftree t n v `2*k+2`))
-   -> (inftree t n v k).
+Inductive inftree (t:array Z) (n v:Z) : Z -> Prop :=
+    inftree_cons :
+      forall k:Z,
+        (0 <= k <= n)%Z ->
+        (access t k <= v)%Z ->
+        ((2 * k + 1 <= n)%Z -> inftree t n v (2 * k + 1)%Z) ->
+        ((2 * k + 2 <= n)%Z -> inftree t n v (2 * k + 2)%Z) ->
+        inftree t n v k.
 
 (* Some lemmas about inftree *)
 
-Lemma inftree_1 : (t:(array Z))(n,v,k:Z)
-  (inftree t n v k) -> `(access t k) <= v`.
+Lemma inftree_1 :
+ forall (t:array Z) (n v k:Z), inftree t n v k -> (access t k <= v)%Z.
 Proof.
-Intros t n v k H. Elim H; Auto.
-Save.
+intros t n v k H.
+ elim H; auto.
+Qed.
 
-Lemma inftree_id : (t1,t2:(array Z))(n,v,k:Z)
-    (inftree t1 n v k)
- -> ((i:Z) `k <= i <= n` -> `(access t1 i) = (access t2 i)`)
- -> (inftree t2 n v k).
+Lemma inftree_id :
+ forall (t1 t2:array Z) (n v k:Z),
+   inftree t1 n v k ->
+   (forall i:Z, (k <= i <= n)%Z -> access t1 i = access t2 i) ->
+   inftree t2 n v k.
 Proof.
-Intros t1 t2 n v k H. Elim H; Intros.
-Apply inftree_cons.
-Assumption.
+intros t1 t2 n v k H.
+ elim H; intros.
+apply inftree_cons.
+assumption.
 
-Rewrite <- (H6 k0). Assumption. Omega'.
+rewrite <- (H6 k0).
+ assumption.
+ Omega'.
 
-Intro. Apply H3. Assumption.
-Intros i Hi. Apply H6; Omega'.
+intro.
+ apply H3.
+ assumption.
+intros i Hi.
+ apply H6; Omega'.
 
-Intro. Apply H5. Assumption.
-Intros i Hi. Apply H6; Omega'.
-Save.
+intro.
+ apply H5.
+ assumption.
+intros i Hi.
+ apply H6; Omega'.
+Qed.
 
-Lemma inftree_2 : (t1,t2:(array Z))(n,v,k,j:Z)
-    `n < (array_length t1)`
- -> (inftree t1 n v j) 
- -> (exchange t2 t1 k j)
- -> `k < j`
- -> `(access t1 k) <= (access t1 j)`
- -> (inftree t2 n v j).
+Lemma inftree_2 :
+ forall (t1 t2:array Z) (n v k j:Z),
+   (n < array_length t1)%Z ->
+   inftree t1 n v j ->
+   exchange t2 t1 k j ->
+   (k < j)%Z -> (access t1 k <= access t1 j)%Z -> inftree t2 n v j.
 Proof.
-Intros t1 t2 n v k j Hn H. Case H.
-Intros.
-Apply inftree_cons.
-Assumption.
-Decompose [exchange] H4. Omega'.
+intros t1 t2 n v k j Hn H.
+ case H.
+intros.
+apply inftree_cons.
+assumption.
+decompose [exchange] H4.
+ Omega'.
 
-Intro. Apply inftree_id with t1:=t1. Auto.
-Decompose [exchange] H4.
-Intros i Hi. Symmetry. Apply H13.
-Omega'. Omega'. Omega'.
+intro.
+ apply inftree_id with (t1 := t1).
+ auto.
+decompose [exchange] H4.
+intros i Hi.
+ symmetry.
+ apply H13.
+Omega'.
+ Omega'.
+ Omega'.
 
-Intro. Apply inftree_id with t1:=t1. Auto.
-Decompose [exchange] H4.
-Intros i Hi. Symmetry. Apply H13.
-Omega'. Omega'. Omega'.
-Save.
+intro.
+ apply inftree_id with (t1 := t1).
+ auto.
+decompose [exchange] H4.
+intros i Hi.
+ symmetry.
+ apply H13.
+Omega'.
+ Omega'.
+ Omega'.
+Qed.
 
-Lemma inftree_trans : (t:(array Z))(n,k,v,v':Z)
-  `v <= v'` -> (inftree t n v k) -> (inftree t n v' k).
+Lemma inftree_trans :
+ forall (t:array Z) (n k v v':Z),
+   (v <= v')%Z -> inftree t n v k -> inftree t n v' k.
 Proof.
-Intros t n k v v' Hvv' H.
-(Elim H; Intros).
-Apply inftree_cons.
-Assumption. Omega'. Auto. Auto.
-Save.
+intros t n k v v' Hvv' H.
+elim H; intros.
+apply inftree_cons.
+assumption.
+ Omega'.
+ auto.
+ auto.
+Qed.
 
-Lemma inftree_3 : (t:(array Z))(n,k:Z)
-  (heap t n k) -> (inftree t n #t[k] k).
+Lemma inftree_3 :
+ forall (t:array Z) (n k:Z), heap t n k -> inftree t n (access t k) k.
 Proof.
-Intros t n k H. Elim H; Intros.
-Apply inftree_cons.
-Assumption.
-Auto with zarith.
-Intro. Apply inftree_trans with v:=#t[`2*k0+1`] v':=#t[k0].  
-Omega'. Auto.
-Intro. Apply inftree_trans with v:=#t[`2*k0+2`] v':=#t[k0].  
-Omega'. Auto.
-Save.
+intros t n k H.
+ elim H; intros.
+apply inftree_cons.
+assumption.
+auto with zarith.
+intro.
+ apply inftree_trans with
+  (v := access t (2 * k0 + 1)) (v' := access t k0).
+  Omega'.
+ auto.
+intro.
+ apply inftree_trans with
+  (v := access t (2 * k0 + 2)) (v' := access t k0).
+  Omega'.
+ auto.
+Qed.
 
-Lemma inftree_all : (t:(array Z))(n,v:Z)
-  (inftree t n v `0`) -> (i:Z)`0 <= i <= n` -> (inftree t n v i).
+Lemma inftree_all :
+ forall (t:array Z) (n v:Z),
+   inftree t n v 0 -> forall i:Z, (0 <= i <= n)%Z -> inftree t n v i.
 Proof.
-Intros t n v H0 i H.
-Generalize H.
-Pattern i.
-Apply heap_induction.
-Auto.
+intros t n v H0 i H.
+generalize H.
+pattern i.
+apply heap_induction.
+auto.
 
-Intros.
-Elim (Z_le_gt_dec k n).
-Intro.
-Generalize H1 a.
-(Case H2; Intros).
-Intuition.
+intros.
+elim (Z_le_gt_dec k n).
+intro.
+generalize H1 a.
+case H2; intros.
+intuition.
 
-Split.
-(Intro; Apply H5; Omega).
-(Intro; Apply H6; Omega).
+split.
+intro; apply H5; omega.
+intro; apply H6; omega.
 
-Intro. (Split; Intro; Absurd `k > n`; Omega).
-Intuition.
-Save.
+intro.
+ split; intro; absurd (k > n)%Z; omega.
+intuition.
+Qed.
 
-Lemma inftree_0_right : (t:(array Z))(n,v:Z)
-  (inftree t n v `0`) -> (i:Z)`0 <= i <= n` -> `(access t i) <= v`.
+Lemma inftree_0_right :
+ forall (t:array Z) (n v:Z),
+   inftree t n v 0 ->
+   forall i:Z, (0 <= i <= n)%Z -> (access t i <= v)%Z.
 Proof.
-Intros t n v H.
-Generalize (inftree_all H).
-Intros.
-Apply inftree_1 with n:=n.
-Exact (H0 i H1).
-Save.
+intros t n v H.
+generalize (inftree_all H).
+intros.
+apply inftree_1 with (n := n).
+exact (H0 i H1).
+Qed.
 
-Lemma inftree_0_left : (t:(array Z))(n,v:Z)
-  `0 <= n` -> 
-  ((i:Z)`0 <= i <= n` -> `(access t i) <= v`) -> (inftree t n v `0`).
+Lemma inftree_0_left :
+ forall (t:array Z) (n v:Z),
+   (0 <= n)%Z ->
+   (forall i:Z, (0 <= i <= n)%Z -> (access t i <= v)%Z) ->
+   inftree t n v 0.
 Proof.
-Intros.
-Cut (i:Z)`0 <= i <= n`->(inftree t n v i).
-Intro.
-(Apply H1; Omega).
+intros.
+cut (forall i:Z, (0 <= i <= n)%Z -> inftree t n v i).
+intro.
+apply H1; omega.
 
-Intros i Hi. Generalize Hi.
-Replace i with `n-(n-i)`.
-Pattern `n-i`.
-Apply Z_lt_induction.
-Intros.
-Apply inftree_cons.
-Assumption.
+intros i Hi.
+ generalize Hi.
+replace i with (n - (n - i))%Z.
+pattern (n - i)%Z.
+apply Z_lt_induction.
+intros.
+apply inftree_cons.
+assumption.
 
-(Apply H0; Omega).
+apply H0; omega.
 
-Intro.
-Replace `2*(n-x)+1` with `n-(n-(2*(n-x)+1))`.
-(Apply H1; Omega).
-Omega.
+intro.
+replace (2 * (n - x) + 1)%Z with (n - (n - (2 * (n - x) + 1)))%Z.
+apply H1; omega.
+omega.
 
-Intro.
-Replace `2*(n-x)+2` with `n-(n-(2*(n-x)+2))`.
-(Apply H1; Omega).
-Omega.
+intro.
+replace (2 * (n - x) + 2)%Z with (n - (n - (2 * (n - x) + 2)))%Z.
+apply H1; omega.
+omega.
 
-Omega. Omega.
-Save.
+omega.
+ omega.
+Qed.
 
-Lemma inftree_exchange : (t1,t2:(array Z))(n,v:Z)
-    `n < (array_length t1)`
- -> (inftree t1 n v `0`) 
- -> (exchange t2 t1 `0` n)
- -> (inftree t2 n v `0`).
+Lemma inftree_exchange :
+ forall (t1 t2:array Z) (n v:Z),
+   (n < array_length t1)%Z ->
+   inftree t1 n v 0 -> exchange t2 t1 0 n -> inftree t2 n v 0.
 Proof.
-Intros.
-Apply inftree_0_left.
-Decompose [exchange] H1.
-Omega.
+intros.
+apply inftree_0_left.
+decompose [exchange] H1.
+omega.
 
-Generalize (inftree_0_right H0).
-Intros.
-Decompose [exchange] H1.
-(Elim (Z_lt_ge_dec `0` i); Intro).
-(Elim (Z_lt_ge_dec i n); Intro).
-Rewrite (H9 i).
-(Apply H2; Omega).
+generalize (inftree_0_right H0).
+intros.
+decompose [exchange] H1.
+elim (Z_lt_ge_dec 0 i); intro.
+elim (Z_lt_ge_dec i n); intro.
+rewrite (H9 i).
+apply H2; omega.
 
-Omega. Omega. Omega.
+omega.
+ omega.
+ omega.
 
-Replace i with n.
-Rewrite H8.
-(Apply H2; Omega).
+replace i with n.
+rewrite H8.
+apply H2; omega.
 
-Omega.
+omega.
 
-Replace i with `0`.
-Rewrite H7.
-(Apply H2; Omega).
+replace i with 0%Z.
+rewrite H7.
+apply H2; omega.
 
-Omega.
-Save.
+omega.
+Qed.
 
-Lemma inftree_weakening : (t:(array Z))(n,v,k:Z)
-  `1 <= n < (array_length t)` -> (inftree t n v k) -> `k <= n-1` -> (inftree t `n-1` v k).
+Lemma inftree_weakening :
+ forall (t:array Z) (n v k:Z),
+   (1 <= n < array_length t)%Z ->
+   inftree t n v k -> (k <= n - 1)%Z -> inftree t (n - 1) v k.
 Proof.
-Intros t n v k Hn Htree.
-Elim Htree; Intros.
-Apply inftree_cons.
-Omega.
-Assumption.
-Intro; Apply H2; Omega.
-Intro; Apply H4; Omega.
-Save.
+intros t n v k Hn Htree.
+elim Htree; intros.
+apply inftree_cons.
+omega.
+assumption.
+intro; apply H2; omega.
+intro; apply H4; omega.
+Qed.
