examples/kmp/Lex.v
@@ -1,4 +1,4 @@
-(**************************************************************************)
+(* Load Programs. *)(**************************************************************************)
 (*                                                                        *)
 (* Proof of the Knuth-Morris-Pratt Algorithm.                             *)
 (*                                                                        *)
@@ -11,39 +11,40 @@
  * order relation. *)
 
 Require Export Relation_Operators.
-Require Lexicographic_Product.
+Require Import Lexicographic_Product.
 
-Implicit Arguments On.
+Set Implicit Arguments.
+Unset Strict Implicit.
 
 Section lexico.
 
-Variable A,B : Set.
+Variables A B : Set.
 
-Variable Ra : A->A->Prop.
-Variable Rb : B->B->Prop.
+Variable Ra : A -> A -> Prop.
+Variable Rb : B -> B -> Prop.
 
-Definition lex := (lexprod A [_:A]B Ra [_:A]Rb).
+Definition lex := lexprod A (fun _:A => B) Ra (fun _:A => Rb).
 
 Lemma lex_well_founded :
-  (well_founded A Ra) -> (well_founded B Rb) ->
-  (well_founded {_:A & B} lex).
+ well_founded Ra -> well_founded Rb -> well_founded lex.
 Proof.
-Intros wfa wfb.
-Exact (wf_lexprod A [_:A]B Ra [_:A]Rb wfa [_]wfb).
-Save.
+intros wfa wfb.
+exact
+ (wf_lexprod A (fun _:A => B) Ra (fun _:A => Rb) wfa (fun _ => wfb)).
+Qed.
 
 End lexico.
 
 (* Instantiation on Z x Z *)
 
-Require ZArith.
-Require Zwf.
+Require Import ZArith.
+Require Import Zwf.
 
-Definition prodZZ := {_:Z & Z}.
+Definition prodZZ := {x_ : Z &  Z}.
 
-Definition pairZ : Z -> Z -> prodZZ := [x,y:Z](existS Z [_:Z]Z x y).
+Definition pairZ (x y:Z) : prodZZ := existS (fun _:Z => Z) x y.
 
-Definition lexZ := (lex (Zwf `0`) (Zwf `0`)).
+Definition lexZ := lex (Zwf 0) (Zwf 0).
 
 Definition lexZ_well_founded :=
-  (lex_well_founded (Zwf_well_founded `0`) (Zwf_well_founded `0`)).
+  lex_well_founded (Zwf_well_founded 0) (Zwf_well_founded 0).
