examples/linked-lists/LinkedLists.v
@@ -1,10 +1,10 @@
-
-Require Why.
+(* Load Programs. *)
+Require Import Why.
 Require Export PolyList.
 
 (** the Coq pointer list associated to a (finite) linked list *)
 
-Definition plist := (list pointer).
+Definition plist := list pointer.
 
 
 (** * Paths *)
@@ -13,11 +13,14 @@ Definition plist := (list pointer).
     there is a path from pointer [p1] to pointer [p2] using links in store [t],
     and the list of pointers along this path is [l]. *)
 
-Inductive lpath [t:pointer_store] : pointer -> plist -> pointer -> Prop :=
-  | Path_null : (p:pointer)(lpath t p (nil pointer) p)
-  | Path_cons : (p1,p2:pointer) (is_valid_pointer t p1) ->
-                (l:(list pointer))(lpath t (pget t p1) l p2) ->
-                (lpath t p1 (cons p1 l) p2).
+Inductive lpath (t:pointer_store) :
+pointer -> plist -> pointer -> Prop :=
+  | Path_null : forall p:pointer, lpath t p nil p
+  | Path_cons :
+      forall p1 p2:pointer,
+        is_valid_pointer t p1 ->
+        forall l:list pointer,
+          lpath t (pget t p1) l p2 -> lpath t p1 (cons p1 l) p2.
 
 Hint lpath : core := Constructors lpath.
 
@@ -27,216 +30,218 @@ Hint lpath : core := Constructors lpath.
 (** [(llist t p l)]: there is a (finite) linked list starting from pointer [p]
     using links in store [t], and this list of pointers is [l] *)
 
-Definition llist [t:pointer_store; p:pointer; l:plist] := (lpath t p l null).
+Definition llist (t:pointer_store) (p:pointer) (l:plist) :=
+  lpath t p l null.
 
-Hints Unfold llist.
+Hints Unfold llist .
 
 (** inductive characterization of [llist] (which could have been an
     inductive definition of [llist])  *)
 
-Lemma llist_null : 
-  (t:pointer_store)(p:pointer)(llist t p (nil pointer)) -> p=null.
+Lemma llist_null :
+ forall (t:pointer_store) (p:pointer), llist t p nil -> p = null.
 Proof.
-Unfold llist; Inversion 1; Trivial.
-Save.
+unfold llist; inversion 1; trivial.
+Qed.
 
-Lemma llist_cons : 
-  (t:pointer_store)(p1,p2:pointer)(l:plist)
-  (llist t p1 (cons p2 l)) -> p1 = p2 /\ (llist t (pget t p2) l).
+Lemma llist_cons :
+ forall (t:pointer_store) (p1 p2:pointer) (l:plist),
+   llist t p1 (cons p2 l) -> p1 = p2 /\ llist t (pget t p2) l.
 Proof.
-Unfold llist; Inversion 1; Intuition.
-Save.
+unfold llist; inversion 1; intuition.
+Qed.
 
 (** invariance of a list when updating a cell outside of this list *)
 
-Lemma llist_pset_same : 
-  (t:pointer_store)(p:pointer)(l:plist)(llist t p l) -> 
-  (p1,p2:pointer) (is_valid_pointer t p1) -> ~(In p1 l) -> 
-  (llist (pset t p1 p2) p l).
+Lemma llist_pset_same :
+ forall (t:pointer_store) (p:pointer) (l:plist),
+   llist t p l ->
+   forall p1 p2:pointer,
+     is_valid_pointer t p1 -> ~ In p1 l -> llist (pset t p1 p2) p l.
 Proof.
-Unfold llist; Induction 1; Intuition.
-Apply Path_cons; Auto.
-Rewrite PointerStore.get_set_other; Auto.
-Auto with *.
-Red; Intro; Apply H4; Subst p0; Auto with *.
-Save.
-Hints Resolve llist_pset_same.
+unfold llist; oldinduction 1; intuition.
+apply Path_cons; auto.
+ rewrite PointerStore.get_set_other; auto.
+auto with *.
+red; intro; apply H4; subst p0; auto with *.
+Qed.
+Hints Resolve llist_pset_same .
 
 (** [llist] is a function *)
 
-Lemma llist_function : 
-  (t:pointer_store)(l1,l2:plist)(p:pointer)
-  (llist t p l1) -> (llist t p l2) -> l1=l2.
+Lemma llist_function :
+ forall (t:pointer_store) (l1 l2:plist) (p:pointer),
+   llist t p l1 -> llist t p l2 -> l1 = l2.
 Proof.
-Induction l1; Intuition.
-Inversion H; Subst.
-Inversion H0; Intuition.
-Inversion H1.
-Inversion H0; Subst.
-Inversion H1; Subst.
-Inversion H5.
-Apply (f_equal ? ? (cons a)).
-Apply H with (pget t a); Auto.
-Save.
+oldinduction l1; intuition.
+inversion H; subst.
+inversion H0; intuition.
+inversion H1.
+inversion H0; subst.
+inversion H1; subst.
+inversion H5.
+apply (f_equal (cons a)).
+apply H with (pget t a); auto.
+Qed.
 
-Lemma llist_append : 
-  (t:pointer_store)(l1,l2:plist)(p:pointer)
-  (llist t p (app l1 l2)) -> 
-  (EX p':pointer | (lpath t p l1 p') /\ (llist t p' l2)).
+Lemma llist_append :
+ forall (t:pointer_store) (l1 l2:plist) (p:pointer),
+   llist t p (app l1 l2) ->
+    EX p' : pointer | lpath t p l1 p' /\ llist t p' l2.
 Proof.
-Induction l1; Simpl; Intuition.
-Exists p; Auto.
-Inversion H0; Subst.
-Elim (H l2 (pget t a) H6); Intuition.
-Exists x; Auto.
-Save.
+oldinduction l1; simpl; intuition.
+exists p; auto.
+inversion H0; subst.
+elim (H l2 (pget t a) H6); intuition.
+exists x; auto.
+Qed.
 
 (** this should go in PolyList *)
-Lemma In_app_cons : 
-  (A:Set)(l:(list A))(x:A) (In x l) -> 
-  (EX l1 : (list A) | (EX l2 : (list A) | l = (app l1 (cons x l2)))).
+Lemma In_app_cons :
+ forall (A:Set) (l:list A) (x:A),
+   In x l ->
+    EX l1 : list A | ( EX l2 : list A | l = app l1 (cons x l2)).
 Proof.
-Induction l; Simpl; Intuition.
-Exists (nil A); Exists l0; Simpl; Subst; Auto.
-Elim (H x H1); Clear H; Intros.
-Elim H; Clear H; Intuition.
-Exists (cons a x0); Exists x1; Simpl; Subst; Auto.
-Save.
+oldinduction l; simpl; intuition.
+exists (nil (A:=A)); exists l0; simpl; subst; auto.
+elim (H x H1); clear H; intros.
+elim H; clear H; intuition.
+exists (cons a x0); exists x1; simpl; subst; auto.
+Qed.
 
-Lemma list_length_absurd : (A:Set)(l1,l2:(list A))
-  ~(length l1)=(length l2) -> ~l1=l2.
+Lemma list_length_absurd :
+ forall (A:Set) (l1 l2:list A), length l1 <> length l2 -> l1 <> l2.
 Proof.
-Induction l1; Induction l2; Simpl; Intuition.
-Discriminate H1.
-Discriminate H1.
-Injection H2; Intros.
-Apply (H l0); Intuition.
-Save.
+oldinduction l1; oldinduction l2; simpl; intuition.
+discriminate H1.
+discriminate H1.
+injection H2; intros.
+apply (H l0); intuition.
+Qed.
 
-Lemma length_app : (A:Set)(l1,l2:(list A))
-  (length (app l1 l2)) = (plus (length l1) (length l2)).
+Lemma length_app :
+ forall (A:Set) (l1 l2:list A),
+   length (app l1 l2) = (length l1 + length l2)%N.
 Proof.
-Induction l1; Simpl; Intuition.
-Save.
+oldinduction l1; simpl; intuition.
+Qed.
 
 (** a list starting with [p] does not contain [p] in its remaining elements *)
 
-Lemma llist_not_starting : 
-  (t:pointer_store)(p:pointer)(l:plist)
-  (llist t (pget t p) l) -> ~(In p l).
+Lemma llist_not_starting :
+ forall (t:pointer_store) (p:pointer) (l:plist),
+   llist t (pget t p) l -> ~ In p l.
 Proof.
-Red; Intros.
-Elim (In_app_cons ? l p H0); Intros.
-Elim H1; Clear H1; Intros.
-Subst l.
-Elim (llist_append t x (cons p x0) (pget t p) H); Intuition.
-Inversion H3; Subst.
-Generalize (llist_function t x0 (app x (cons p x0)) (pget t p) H8 H).
-Intro; Apply (list_length_absurd ? x0 (app x (cons p x0))); Auto.
-Rewrite length_app; Simpl; Omega.
-Save.
+red; intros.
+elim (In_app_cons _ l p H0); intros.
+elim H1; clear H1; intros.
+subst l.
+elim (llist_append t x (cons p x0) (pget t p) H); intuition.
+inversion H3; subst.
+generalize (llist_function t x0 (app x (cons p x0)) (pget t p) H8 H).
+intro; apply (list_length_absurd _ x0 (app x (cons p x0))); auto.
+rewrite length_app; simpl; omega.
+Qed.
 
 
 (** * Finite lists characterization *)
 
-Inductive is_list [t: pointer_store] : pointer -> Prop :=
-  | List_null : (is_list t null)
-  | List_cons : (p:pointer) (is_valid_pointer t p) -> 
-                (is_list t (pget t p)) -> (is_list t p).
+Inductive is_list (t:pointer_store) : pointer -> Prop :=
+  | List_null : is_list t null
+  | List_cons :
+      forall p:pointer,
+        is_valid_pointer t p -> is_list t (pget t p) -> is_list t p.
 
 Hint is_list : core := Constructors is_list.
 
-Lemma is_list_llist : 
-  (t:pointer_store)
-  (p:pointer)(is_list t p) -> (EX l:plist | (llist t p l)).
+Lemma is_list_llist :
+ forall (t:pointer_store) (p:pointer),
+   is_list t p ->  EX l : plist | llist t p l.
 Proof.
-Intros; Induction H.
-Exists (nil pointer); Intuition.
-Elim HrecH; Intros.
-Exists (cons p x); Intuition.
-Save.
+intros; oldinduction H.
+exists (nil (A:=pointer)); intuition.
+elim HrecH; intros.
+exists (cons p x); intuition.
+Qed.
 
 Lemma llist_is_list :
-  (t:pointer_store)
-  (l:plist)(p:pointer)(llist t p l) -> (is_list t p).
+ forall (t:pointer_store) (l:plist) (p:pointer),
+   llist t p l -> is_list t p.
 Proof.
-Induction l; Intuition.
-Inversion H; Auto.
-Inversion H0; Intuition.
-Save.
+oldinduction l; intuition.
+inversion H; auto.
+inversion H0; intuition.
+Qed.
 
 
 (** * WF relation over linked lists *)
 
 Definition StorePointerPair := pointer_store * pointer.
-Definition store_pointer_pair := [t:pointer_store; p:pointer](t, p).
+Definition store_pointer_pair (t:pointer_store) (p:pointer) := (t, p).
 
-Definition ll_order [c1,c2: pointer_store * pointer] : Prop :=
-  let (t1,p1) = c1 in
-  let (t2,p2) = c2 in
-  (EX l1:plist | (EX l2:plist | 
-    (llist t1 p1 l1) /\ (llist t2 p2 l2) /\ 
-    (lt (length l1) (length l2)))).
+Definition ll_order (c1 c2:pointer_store * pointer) : Prop :=
+  let (t1, p1) := c1 in
+  let (t2, p2) := c2 in
+   EX l1 : plist
+  | ( EX l2 : plist
+     | llist t1 p1 l1 /\ llist t2 p2 l2 /\ (length l1 < length l2)%N).
 
-Lemma ll_order_wf : (well_founded ll_order).
+Lemma ll_order_wf : well_founded ll_order.
 Proof.
-Apply well_founded_inv_lt_rel_compat
-  with F := [x:StorePointerPair][n]
-            (let (t,p) = x in 
-            (EX l:plist | (llist t p l) /\ (length l)=n)).
-Unfold ll_order inv_lt_rel.
-Destruct x; Destruct y; Intuition.
-Elim H; Clear H; Intros l1 H; Elim H; Clear H; Intros l2 H.
-Intuition.
-Exists (length l1).
-Exists l1; Intuition.
-Intuition.
-Elim H1; Intros l2'; Intuition.
-Generalize (llist_function ? ?? ? H H4); Intro; Subst l2.
-Omega.
-Save.
-Hints Resolve ll_order_wf.
+apply well_founded_inv_lt_rel_compat with
+ (F := fun (x:StorePointerPair) n =>
+         let (t, p) := x in  EX l : plist | llist t p l /\ length l = n).
+unfold ll_order, inv_lt_rel.
+olddestruct x; olddestruct y; intuition.
+elim H; clear H; intros l1 H; elim H; clear H; intros l2 H.
+intuition.
+exists (length l1).
+exists l1; intuition.
+intuition.
+elim H1; intros l2'; intuition.
+generalize (llist_function _ _ _ _ H H4); intro; subst l2.
+omega.
+Qed.
+Hints Resolve ll_order_wf .
 
 
 (** * Disjointness *)
 
 (** [disjoint l1 l2]: no common element between lists [l1] and [l2] *)
 
-Definition disjoint [A:Set; l1,l2:(list A)] : Prop :=
-  ((x:A)(In x l1) -> ~(In x l2)) /\
-  ((x:A)(In x l2) -> ~(In x l1)).
-Implicits disjoint.
+Definition disjoint (A:Set) (l1 l2:list A) : Prop :=
+  (forall x:A, In x l1 -> ~ In x l2) /\
+  (forall x:A, In x l2 -> ~ In x l1).
+Implicit Arguments disjoint.
 
 Section Disjointness.
 
 Variable A : Set.
-Variable l1,l2 : (list A).
+Variables l1 l2 : list A.
 Variable x : A.
 
-Lemma disjoint_cons : 
-  (disjoint l1 (cons x l2)) -> 
-  ~(In x l2) ->
-  (disjoint (cons x l1) l2).
+Lemma disjoint_cons :
+ disjoint l1 (cons x l2) -> ~ In x l2 -> disjoint (cons x l1) l2.
 Proof.
-Unfold disjoint; Intuition.
-Elim (in_inv H); Intuition.
-Subst x; Intuition.
-Apply H1 with x0; Intuition.
-Elim (in_inv H3); Intuition.
-Subst x; Intuition.
-Apply H1 with x0; Intuition.
-Save.
+unfold disjoint; intuition.
+elim (in_inv H); intuition.
+subst x; intuition.
+apply H1 with x0; intuition.
+elim (in_inv H3); intuition.
+subst x; intuition.
+apply H1 with x0; intuition.
+Qed.
 
-Lemma disjoint_nil_l : (disjoint (nil A) l2).
+Lemma disjoint_nil_l : disjoint nil l2.
 Proof.
-Unfold disjoint; Intuition.
-Save.
+unfold disjoint; intuition.
+Qed.
 
-Lemma disjoint_l_nil : (disjoint l1 (nil A)).
+Lemma disjoint_l_nil : disjoint l1 nil.
 Proof.
-Unfold disjoint; Intuition.
-Save.
+unfold disjoint; intuition.
+Qed.
 
 End Disjointness.
-Hints Resolve disjoint_cons disjoint_nil_l disjoint_l_nil.
+Hints Resolve disjoint_cons disjoint_nil_l disjoint_l_nil .
 
