examples/quicksort/Partition.v
@@ -1,4 +1,4 @@
-(**************************************************************************)
+(* Load Programs. *)(**************************************************************************)
 (*                                                                        *)
 (* Proof of the Quicksort Algorithm.                                      *)
 (*                                                                        *)
@@ -7,14 +7,15 @@
 (*                                                                        *)
 (**************************************************************************)
 
-Require Why.
+Require Import Why.
 
-Require Omega.
+Require Import Omega.
 
-Implicit Arguments On.
+Set Implicit Arguments.
+Unset Strict Implicit.
 
 
-(* Here we define the property "partition_p" which expresses that,
+(* Here we define the property  which expresses that,
  * on the segment [g,d] of the array t, all elements on the left of p
  * are lesser or equal than t[p] and all elements on the right of p
  * are greater or equal than t[p].
@@ -23,169 +24,182 @@ Implicit Arguments On.
  * that all elements of a segment [g,d] are <= (resp. >=) than a given value
  *)
 
-Inductive array_le [t:(array Z) ; g,d,v:Z] : Prop
-  := array_le_cons :
-     ((i:Z) `g <= i <= d` -> (Zle #t[i] v))
-  -> (array_le t g d v).
+Inductive array_le (t:array Z) (g d v:Z) : Prop :=
+    array_le_cons :
+      (forall i:Z, (g <= i <= d)%Z -> (access t i <= v)%Z) ->
+      array_le t g d v.
 
-Inductive array_ge [t:(array Z) ; g,d,v:Z] : Prop
-  := array_ge_cons :
-     ((i:Z) `g <= i <= d` -> (Zle v #t[i]))
-  -> (array_ge t g d v).
+Inductive array_ge (t:array Z) (g d v:Z) : Prop :=
+    array_ge_cons :
+      (forall i:Z, (g <= i <= d)%Z -> (v <= access t i)%Z) ->
+      array_ge t g d v.
 
-Inductive partition_p [t:(array Z) ; g,d,p:Z] : Prop
-  := piv : `g <= p` -> `p <= d`
-         -> (array_le t g `p-1` #t[p])
-         -> (array_ge t `p+1` d #t[p])
-         -> (partition_p t g d p).
+Inductive partition_p (t:array Z) (g d p:Z) : Prop :=
+    piv :
+      (g <= p)%Z ->
+      (p <= d)%Z ->
+      array_le t g (p - 1) (access t p) ->
+      array_ge t (p + 1) d (access t p) -> partition_p t g d p.
 
 
 (* Lemmas about array_le *)
 
 Lemma array_le_empty :
-  (t:(array Z))(g,d,v:Z)
-    `d < g`
-    -> (array_le t g d v).
+ forall (t:array Z) (g d v:Z), (d < g)%Z -> array_le t g d v.
 Proof.
-Intros t g d v H.
-Constructor. Intros.
-Absurd `g<=d`; Omega.
-Save.
+intros t g d v H.
+constructor.
+ intros.
+absurd (g <= d)%Z; omega.
+Qed.
 
 Lemma array_le_right_extension :
-  (t:(array Z))(g,d,v:Z)
-    (array_le t g d v)
-    -> (Zle #t[`d+1`] v)
-      -> (array_le t g `d+1` v).
+ forall (t:array Z) (g d v:Z),
+   array_le t g d v ->
+   (access t (d + 1) <= v)%Z -> array_le t g (d + 1) v.
 Proof.
-Intros t g d v H_le Hv.
-Elim H_le; Intros.
-Constructor. Intros.
-Elim (Z_eq_dec i `d+1`); Intro.
-Rewrite a; Assumption.
-Apply H; Omega.
-Save.
+intros t g d v H_le Hv.
+elim H_le; intros.
+constructor.
+ intros.
+elim (Z_eq_dec i (d + 1)); intro.
+rewrite a; assumption.
+apply H; omega.
+Qed.
 
 Lemma array_le_exchange :
-  (t,t':(array Z))(g,d,v:Z)(x,y:Z)
-    `0 <= g` -> `d < (array_length t)`
-    -> (array_le t g d v)
-    -> `d < x <= y`
-      -> (exchange t t' x y)
-        -> (array_le t' g d v).
+ forall (t t':array Z) (g d v x y:Z),
+   (0 <= g)%Z ->
+   (d < array_length t)%Z ->
+   array_le t g d v ->
+   (d < x <= y)%Z -> exchange t t' x y -> array_le t' g d v.
 Proof.
-Intros t t' g d v x y Hg Hd Hle Hxy Hex.
-Elim Hle; Intros. 
-Elim Hex; Intros.
-Constructor. Intros.
-Rewrite <- H5; Try Omega.
-Apply H; Assumption.
-Save.
+intros t t' g d v x y Hg Hd Hle Hxy Hex.
+elim Hle; intros.
+ elim Hex; intros.
+constructor.
+ intros.
+rewrite <- H5; try omega.
+apply H; assumption.
+Qed.
 
 (* Lemmas about array_ge *)
 
 Lemma array_ge_empty :
-  (t:(array Z))(g,d,v:Z)
-    `d < g`
-    -> (array_ge t g d v).
+ forall (t:array Z) (g d v:Z), (d < g)%Z -> array_ge t g d v.
 Proof.
-Intros t g d v H.
-Constructor. Intros.
-Absurd `g<=d`; Omega.
-Save.
+intros t g d v H.
+constructor.
+ intros.
+absurd (g <= d)%Z; omega.
+Qed.
 
 Lemma array_ge_left_extension :
-  (t:(array Z))(g,d,v:Z)
-    (array_ge t g d v)
-    -> (Zle v #t[`g-1`])
-      -> (array_ge t `g-1` d v).
+ forall (t:array Z) (g d v:Z),
+   array_ge t g d v ->
+   (v <= access t (g - 1))%Z -> array_ge t (g - 1) d v.
 Proof.
-Intros t g d v H_ge Hv.
-Elim H_ge; Intros.
-Constructor. Intros.
-Elim (Z_eq_dec i `g-1`); Intro.
-Rewrite a; Assumption.
-Apply H; Omega.
-Save.
+intros t g d v H_ge Hv.
+elim H_ge; intros.
+constructor.
+ intros.
+elim (Z_eq_dec i (g - 1)); intro.
+rewrite a; assumption.
+apply H; omega.
+Qed.
 
 Lemma array_ge_exchange :
-  (t,t':(array Z))(g,d,v:Z)(x,y:Z)
-    `0 <= g` -> `d < (array_length t)`
-    -> (array_ge t g d v)
-    -> `x <= y < g`
-      -> (exchange t t' x y)
-        -> (array_ge t' g d v).
+ forall (t t':array Z) (g d v x y:Z),
+   (0 <= g)%Z ->
+   (d < array_length t)%Z ->
+   array_ge t g d v ->
+   (x <= y < g)%Z -> exchange t t' x y -> array_ge t' g d v.
 Proof.
-Intros t t' g d v x y Hg Hd Hge Hxy Hex.
-Elim Hge; Intros. 
-Elim Hex; Intros.
-Constructor. Intros.
-Rewrite <- H5; Try Omega.
-Apply H; Assumption.
-Save.
+intros t t' g d v x y Hg Hd Hge Hxy Hex.
+elim Hge; intros.
+ elim Hex; intros.
+constructor.
+ intros.
+rewrite <- H5; try omega.
+apply H; assumption.
+Qed.
 
 
 (* Lemmas about partition_p and sub_permut *)
 
 Lemma partition_p_permut_left :
-  (t,t':(array Z))(g,d,p:Z)
-  `0 <= g` -> `g < d` -> `d < (array_length t)` -> `g <= p <= d`
-  -> (partition_p t g d p)
-  -> (sub_permut g (Zpred p) t t')
-  -> (partition_p t' g d p).
+ forall (t t':array Z) (g d p:Z),
+   (0 <= g)%Z ->
+   (g < d)%Z ->
+   (d < array_length t)%Z ->
+   (g <= p <= d)%Z ->
+   partition_p t g d p ->
+   sub_permut g (Zpred p) t t' -> partition_p t' g d p.
 Proof.
-Intros t t' g d p hyp1 hyp2 hyp3 hyp4 piv_t perm.
-Elim piv_t; Intros.
-Cut `(Zpred p)<(array_length t)` ; [ Intro | Unfold Zpred; Omega ].
-Generalize (sub_permut_function perm hyp1 H3). Intro.
-Constructor; Try Assumption.
+intros t t' g d p hyp1 hyp2 hyp3 hyp4 piv_t perm.
+elim piv_t; intros.
+cut (Zpred p < array_length t)%Z; [ intro | unfold Zpred; omega ].
+generalize (sub_permut_function perm hyp1 H3).
+ intro.
+constructor; try assumption.
 (* array_le *)
-Constructor. Intros.
-Rewrite <- (sub_permut_eq perm 7!p).
-Elim H1; Intros.
-Elim (H4 i); Try (Unfold Zpred; Omega). Intros.
-Elim H8; Intros.
-Elim H9; Intros. Rewrite H11.
-Apply H6; Unfold Zpred in H10; Omega.
-Unfold Zpred; Omega.
+constructor.
+ intros.
+rewrite <- (sub_permut_eq perm (i:=p)).
+elim H1; intros.
+elim (H4 i); try (unfold Zpred; omega).
+ intros.
+elim H8; intros.
+elim H9; intros.
+ rewrite H11.
+apply H6; unfold Zpred in H10; omega.
+unfold Zpred; omega.
 (* array_ge *)
-Constructor. Intros.
-Rewrite <- (sub_permut_eq perm 7!p).
-Rewrite <- (sub_permut_eq perm 7!i).
-Elim H2; Intros.
-Apply H6; Omega.
-Unfold Zpred; Omega.
-Unfold Zpred; Omega.
-Save.
+constructor.
+ intros.
+rewrite <- (sub_permut_eq perm (i:=p)).
+rewrite <- (sub_permut_eq perm (i:=i)).
+elim H2; intros.
+apply H6; omega.
+unfold Zpred; omega.
+unfold Zpred; omega.
+Qed.
 
 
 Lemma partition_p_permut_right :
-  (t,t':(array Z))(g,d,p:Z)
-  `0 <= g` -> `g < d` -> `d < (array_length t)` -> `g <= p <= d`
-  -> (partition_p t g d p)
-  -> (sub_permut (Zs p) d t t')
-  -> (partition_p t' g d p).
+ forall (t t':array Z) (g d p:Z),
+   (0 <= g)%Z ->
+   (g < d)%Z ->
+   (d < array_length t)%Z ->
+   (g <= p <= d)%Z ->
+   partition_p t g d p ->
+   sub_permut (Zs p) d t t' -> partition_p t' g d p.
 Proof.
-Intros t t' g d p hyp1 hyp2 hyp3 hyp4 piv_t perm.
-Elim piv_t; Intros.
-Cut `0<=(Zs p)` ; [ Intro | Unfold Zpred; Omega ].
-Generalize (sub_permut_function perm H3 hyp3). Intro.
-Constructor; Try Assumption.
+intros t t' g d p hyp1 hyp2 hyp3 hyp4 piv_t perm.
+elim piv_t; intros.
+cut (0 <= Zs p)%Z; [ intro | unfold Zpred; omega ].
+generalize (sub_permut_function perm H3 hyp3).
+ intro.
+constructor; try assumption.
 (* array_le *)
-Constructor. Intros.
-Rewrite <- (sub_permut_eq perm 7!p).
-Rewrite <- (sub_permut_eq perm 7!i).
-Elim H1; Intros.
-Apply H6; Omega.
-Unfold Zs; Omega.
-Unfold Zs; Omega.
+constructor.
+ intros.
+rewrite <- (sub_permut_eq perm (i:=p)).
+rewrite <- (sub_permut_eq perm (i:=i)).
+elim H1; intros.
+apply H6; omega.
+unfold Zs; omega.
+unfold Zs; omega.
 (* array_ge *)
-Constructor. Intros.
-Rewrite <- (sub_permut_eq perm 7!p).
-Elim H2; Intros.
-Elim (H4 i); Try (Unfold Zs; Omega). Intros.
-Elim H8; Intros.
-Elim H9; Intros. Rewrite H11.
-Apply H6; Unfold Zs in H10; Omega.
-Unfold Zs; Omega.
-Save.
+constructor.
+ intros.
+rewrite <- (sub_permut_eq perm (i:=p)).
+elim H2; intros.
+elim (H4 i); try (unfold Zs; omega).
+ intros.
+elim H8; intros.
+elim H9; intros.
+ rewrite H11.
+apply H6; unfold Zs in H10; omega.
+unfold Zs; omega.
+Qed.
