examples/find/find_proofs.v
@@ -1,11 +1,11 @@
-(**********************************************************************)
+(* Load Programs. *)(**********************************************************************)
 (*                                                                    *)
 (* FIND, an historical example.                                       *)
 (*                                                                    *)
 (* The proof of this program was originally done by C. A. R. Hoare    *)
 (* and fully detailed in the following paper:                         *)
 (*                                                                    *)
-(* C. A. R. Hoare, "Proof of a Program: FIND", Communications of the  *)
+(* C. A. R. Hoare, , Communications of the  *)
 (* ACM, 14(1), 39--45, January 1971.                                  *)
 (*                                                                    *)
 (**********************************************************************)
@@ -14,341 +14,421 @@
 (* find_proofs.v                                                      *)
 (**********************************************************************)
 
-Require find_spec.
-Require find_lemmas.
-Require Why.
-Require Omega.
+Require Import find_spec.
+Require Import find_lemmas.
+Require Import Why.
+Require Import Omega.
 
-Lemma zero_f_SN : `0 <= f < (Zs N)`.
+Lemma zero_f_SN : (0 <= f < Zs N)%Z.
 Proof.
-Generalize le_1_f; Generalize le_f_N; Intros; Omega.
-Save.
+generalize le_1_f; generalize le_f_N; intros; omega.
+Qed.
 
 (* Lemmas to prove arrays bounds obligations. *)
 
-Lemma bound_3 : (m,n,i,r:Z)(A:(array Z))
-  (i_invariant m n i r A) ->
-  `i <= n` ->
-  (Zlt #A[i] r) ->
-  `(Zs i) <= n`.
+Lemma bound_3 :
+ forall (m n i r:Z) (A:array Z),
+   i_invariant m n i r A ->
+   (i <= n)%Z -> (access A i < r)%Z -> (Zs i <= n)%Z.
 Proof.
-Unfold i_invariant.
-Intros m n i r A Hi le_i_n lt_Ai_r.
-Decompose [and] Hi.
-Case (Z_le_lt_eq_dec i n le_i_n).
-Intro. Abstract Omega.
-Intro eq_i_n. Elim (H2 le_i_n). Intros.
-Absurd (Zlt #A[i] r).
-Cut x=i. Intro eq_x_i. Rewrite eq_x_i in H0. Abstract Omega.
-Abstract Omega.
-Assumption.
-Save.
+unfold i_invariant.
+intros m n i r A Hi le_i_n lt_Ai_r.
+decompose [and] Hi.
+case (Z_le_lt_eq_dec i n le_i_n).
+intro.
+ abstract omega.
+intro eq_i_n.
+ elim (H2 le_i_n).
+ intros.
+absurd (access A i < r)%Z.
+cut (x = i).
+ intro eq_x_i.
+ rewrite eq_x_i in H0.
+ abstract omega.
+abstract omega.
+assumption.
+Qed.
 
 
-Lemma bound_4 : (m,n,j,r:Z)(A:(array Z))
-  (j_invariant m n j r A) ->
-  `m <= j` ->
-  (Zlt r #A[j]) ->
-  `m <= (Zpred j)`.
+Lemma bound_4 :
+ forall (m n j r:Z) (A:array Z),
+   j_invariant m n j r A ->
+   (m <= j)%Z -> (r < access A j)%Z -> (m <= Zpred j)%Z.
 Proof.
-Unfold j_invariant.
-Intros m n j r A Hj le_m_j lt_r_Aj.
-Decompose [and] Hj.
-Case (Z_le_lt_eq_dec m j le_m_j).
-Intro. Unfold Zpred. Abstract Omega.
-Intro eq_m_j. Elim (H2 le_m_j). Intros.
-Absurd (Zlt r #A[j]).
-Cut x=j. Intro eq_x_j. Rewrite eq_x_j in H0. Abstract Omega.
-Abstract Omega.
-Assumption.
-Save.
+unfold j_invariant.
+intros m n j r A Hj le_m_j lt_r_Aj.
+decompose [and] Hj.
+case (Z_le_lt_eq_dec m j le_m_j).
+intro.
+ unfold Zpred.
+ abstract omega.
+intro eq_m_j.
+ elim (H2 le_m_j).
+ intros.
+absurd (r < access A j)%Z.
+cut (x = j).
+ intro eq_x_j.
+ rewrite eq_x_j in H0.
+ abstract omega.
+abstract omega.
+assumption.
+Qed.
 
 
 (* Some subgoals of the main proof *)
 
-Lemma subgoal_1 : (m1,n1,i2,j2,i3:Z)(A,A0,A1:(array Z))
-  (m_invariant m1 A0)
-          /\(n_invariant n1 A0)/\(permut A0 A)/\`1 <= m1`/\`n1 <= N` ->
-  `m1 < n1` ->
-  `0 <= f < (Zs N)` ->
-  (i_invariant m1 n1 i2 (#A0[f]) A1)
-    /\ (j_invariant m1 n1 j2 (#A0[f]) A1)
-    /\ (m_invariant m1 A1)/\(n_invariant n1 A1)
-    /\ `0 <= j2`/\`i2 <= N+1`
-    /\(termination i2 j2 m1 n1 (#A0[f]) A1)
-    /\(permut A1 A) ->
-  `i2 <= j2` ->
-  (i_invariant m1 n1 i3 (#A0[f]) A1)
-    /\`i2 <= i3`
-    /\`i3 <= n1` 
-    /\(termination i3 j2 m1 n1 (#A0[f]) A1)->
-  `(access   A1 i3) < (access   A0 f)` ->
-
-  (i_invariant m1 n1 (Zs i3) (#A0[f]) A1)
-   /\ `i2 <= (Zs i3)`
-   /\ `(Zs i3) <= n1`
-   /\ (termination (Zs i3) j2 m1 n1 (#A0[f]) A1).
-
-Proof.
-Intros m1 n1 i2 j2 i3 A A0 A1 HH_43 HH_42 HH_40 HH_28 HH_27 HH_4 HH_2.
-Split.
-Apply Lemma_8_15. Elim HH_4; Auto.
-Decompose [and] HH_4. Elim H. Intros. Abstract Omega.
-Split; [ Abstract Omega | Split ].
-Cut `(Zs i3) <= n1`. Abstract Omega.
-Apply bound_3 with m:=m1 r:=#A0[f] A:=A1; Auto.
-Elim HH_4; Auto. Abstract Omega.
-(* term. *)
-Unfold termination. 
-Decompose [and] HH_4. Elim H3.
-Intro. Left. Abstract Omega.
-Intro. Right. Decompose [and] H2.
-Case (Z_le_lt_eq_dec i3 f H6).
-  Intro. Abstract Omega.
-  Intro eq_i3_f. Absurd `(access   A1 i3) < (access   A0 f)`; Auto.
-  Rewrite eq_i3_f. Abstract Omega.
-Save.
-
-
-Lemma subgoal_2 : (m1,n1,i2,j2,i3,j3:Z)(A,A0,A1:(array Z))
-  (m_invariant m1 A0)
-    /\(n_invariant n1 A0)
-    /\(permut A0 A)
-    /\`1 <= m1`/\`n1 <= N` ->
-  `m1 < n1` ->
-  `0 <= f < (Zs N)` ->
-  (i_invariant m1 n1 i2 (#A0[f]) A1)
-    /\(j_invariant m1 n1 j2 (#A0[f]) A1)
-    /\(m_invariant m1 A1)/\(n_invariant n1 A1)
-    /\`0 <= j2`/\`i2 <= N+1`
-    /\(termination i2 j2 m1 n1 (#A0[f]) A1)
-    /\(permut A1 A) ->
-  `i2 <= j2` ->
-  ((i_invariant m1 n1 i3 (#A0[f]) A1)
-     /\`i2 <= i3`/\`i3 <= n1`
-     /\(termination i3 j2 m1 n1 (#A0[f]) A1))
-    /\`(access   A1 i3) >= (access   A0 f)` ->
-  (j_invariant m1 n1 j3 (#A0[f]) A1)
-    /\`j3 <= j2`/\`m1 <= j3` 
-    /\ (termination i3 j3 m1 n1 (#A0[f]) A1) ->
-  `(access   A0 f) < (access   A1 j3)` ->
-
-  (j_invariant m1 n1 (Zpred j3) (#A0[f]) A1)
-    /\`(Zpred j3) <= j2`/\`m1 <= (Zpred j3)`
-    /\(termination i3 (Zpred j3) m1 n1 (#A0[f]) A1).
+Lemma subgoal_1 :
+ forall (m1 n1 i2 j2 i3:Z) (A A0 A1:array Z),
+   m_invariant m1 A0 /\
+   n_invariant n1 A0 /\ permut A0 A /\ (1 <= m1)%Z /\ (n1 <= N)%Z ->
+   (m1 < n1)%Z ->
+   (0 <= f < Zs N)%Z ->
+   i_invariant m1 n1 i2 (access A0 f) A1 /\
+   j_invariant m1 n1 j2 (access A0 f) A1 /\
+   m_invariant m1 A1 /\
+   n_invariant n1 A1 /\
+   (0 <= j2)%Z /\
+   (i2 <= N + 1)%Z /\
+   termination i2 j2 m1 n1 (access A0 f) A1 /\ permut A1 A ->
+   (i2 <= j2)%Z ->
+   i_invariant m1 n1 i3 (access A0 f) A1 /\
+   (i2 <= i3)%Z /\
+   (i3 <= n1)%Z /\ termination i3 j2 m1 n1 (access A0 f) A1 ->
+   (access A1 i3 < access A0 f)%Z ->
+   i_invariant m1 n1 (Zs i3) (access A0 f) A1 /\
+   (i2 <= Zs i3)%Z /\
+   (Zs i3 <= n1)%Z /\ termination (Zs i3) j2 m1 n1 (access A0 f) A1.
 
 Proof.
-Intros m1 n1 i2 j2 i3 j3 A A0 A1 HH_43 HH_42 HH_40 HH_28 HH_27 
-  HH_25 HH_9 HH_7.
-Split.
-Apply Lemma_9_17. Elim HH_9; Auto.
-Unfold j_invariant in HH_9. Decompose [and] HH_9. Elim H3. Intros. Abstract Omega.
-Assumption.
-Cut `m1 <= (Zpred j3)`. Unfold Zpred. 
- Split ; [ Abstract Omega | Split ; [ Abstract Omega | Idtac ] ].
+intros m1 n1 i2 j2 i3 A A0 A1 HH_43 HH_42 HH_40 HH_28 HH_27 HH_4 HH_2.
+split.
+apply Lemma_8_15.
+ elim HH_4; auto.
+decompose [and] HH_4.
+ elim H.
+ intros.
+ abstract omega.
+split; [ abstract omega | split ].
+cut (Zs i3 <= n1)%Z.
+ abstract omega.
+apply bound_3 with (m := m1) (r := access A0 f) (A := A1); auto.
+elim HH_4; auto.
+ abstract omega.
 (* term. *)
-Unfold termination.
-Decompose [and] HH_9. Elim H4.
-Intro. Left. Abstract Omega.
-Intro. Right. Decompose [and] H3.
-Case (Z_le_lt_eq_dec f j3 H8).
-  Intro. Abstract Omega.
-  Intro eq_f_j3. Absurd `(access   A0 f) < (access   A1 j3)`; Auto.
-  Rewrite <- eq_f_j3. Abstract Omega.
+unfold termination.
+ decompose [and] HH_4.
+ elim H3.
+intro.
+ left.
+ abstract omega.
+intro.
+ right.
+ decompose [and] H2.
+case (Z_le_lt_eq_dec i3 f H6).
+  intro.
+ abstract omega.
+  intro eq_i3_f.
+ absurd (access A1 i3 < access A0 f)%Z; auto.
+  rewrite eq_i3_f.
+ abstract omega.
+Qed.
+
+
+Lemma subgoal_2 :
+ forall (m1 n1 i2 j2 i3 j3:Z) (A A0 A1:array Z),
+   m_invariant m1 A0 /\
+   n_invariant n1 A0 /\ permut A0 A /\ (1 <= m1)%Z /\ (n1 <= N)%Z ->
+   (m1 < n1)%Z ->
+   (0 <= f < Zs N)%Z ->
+   i_invariant m1 n1 i2 (access A0 f) A1 /\
+   j_invariant m1 n1 j2 (access A0 f) A1 /\
+   m_invariant m1 A1 /\
+   n_invariant n1 A1 /\
+   (0 <= j2)%Z /\
+   (i2 <= N + 1)%Z /\
+   termination i2 j2 m1 n1 (access A0 f) A1 /\ permut A1 A ->
+   (i2 <= j2)%Z ->
+   (i_invariant m1 n1 i3 (access A0 f) A1 /\
+    (i2 <= i3)%Z /\
+    (i3 <= n1)%Z /\ termination i3 j2 m1 n1 (access A0 f) A1) /\
+   (access A1 i3 >= access A0 f)%Z ->
+   j_invariant m1 n1 j3 (access A0 f) A1 /\
+   (j3 <= j2)%Z /\
+   (m1 <= j3)%Z /\ termination i3 j3 m1 n1 (access A0 f) A1 ->
+   (access A0 f < access A1 j3)%Z ->
+   j_invariant m1 n1 (Zpred j3) (access A0 f) A1 /\
+   (Zpred j3 <= j2)%Z /\
+   (m1 <= Zpred j3)%Z /\
+   termination i3 (Zpred j3) m1 n1 (access A0 f) A1.
+
+Proof.
+intros m1 n1 i2 j2 i3 j3 A A0 A1 HH_43 HH_42 HH_40 HH_28 HH_27 HH_25
+ HH_9 HH_7.
+split.
+apply Lemma_9_17.
+ elim HH_9; auto.
+unfold j_invariant in HH_9.
+ decompose [and] HH_9.
+ elim H3.
+ intros.
+ abstract omega.
+assumption.
+cut (m1 <= Zpred j3)%Z.
+ unfold Zpred.
+  split; [ abstract omega | split; [ abstract omega | idtac ] ].
+(* term. *)
+unfold termination.
+decompose [and] HH_9.
+ elim H4.
+intro.
+ left.
+ abstract omega.
+intro.
+ right.
+ decompose [and] H3.
+case (Z_le_lt_eq_dec f j3 H8).
+  intro.
+ abstract omega.
+  intro eq_f_j3.
+ absurd (access A0 f < access A1 j3)%Z; auto.
+  rewrite <- eq_f_j3.
+ abstract omega.
 (* *)
-Apply bound_4 with n:=n1 r:=#A0[f] A:=A1; Auto.
-Elim HH_9; Auto. Abstract Omega.
-Save.
+apply bound_4 with (n := n1) (r := access A0 f) (A := A1); auto.
+elim HH_9; auto.
+ abstract omega.
+Qed.
 
 
-Lemma subgoal_3 : (m0,n0,i0,j0,i1,j1:Z)(A,A0,A1,A2:(array Z))
-  `(array_length A)=N+1` -> 
-  (m_invariant m0 A0)
-           /\(n_invariant n0 A0)/\(permut A0 A)/\`1 <= m0`/\`n0 <= N`
- -> `m0 < n0`
- -> `0 <= f < (Zs N)`
- -> (i_invariant m0 n0 i0 (#A0[f]) A1)
-           /\(j_invariant m0 n0 j0 (#A0[f]) A1)
-             /\(m_invariant m0 A1)
-               /\(n_invariant n0 A1)
-                 /\`0 <= j0`
-                   /\`i0 <= N+1`
-                     /\(termination i0 j0 m0 n0 (#A0[f]) A1)
-                       /\(permut A1 A)
- -> `i0 <= j0`
- -> ((i_invariant m0 n0 i1 (#A0[f]) A1)
-           /\`i0 <= i1`
-             /\`i1 <= n0`/\(termination i1 j0 m0 n0 (#A0[f]) A1))
-          /\`(access   A1 i1) >= (access   A0 f)`
- -> ((j_invariant m0 n0 j1 (#A0[f]) A1)
-           /\`j1 <= j0`
-             /\`m0 <= j1`/\(termination i1 j1 m0 n0 (#A0[f]) A1))
-          /\`(access   A0 f) >= (access   A1 j1)`
- -> `(access   A1 j1) <= (access   A0 f) <= (access   A1 i1)`
- -> `i1 <= j1`
- -> (exchange A2 A1 i1 j1)
- -> `(access   A2 i1) <= (access   A0 f)`
- -> `(access   A0 f) <= (access   A2 j1)`
- -> (Zwf `0` `N+2+(Zpred j1)-(Zs i1)` `N+2+j0-i0`)
-   /\(i_invariant m0 n0 (Zs i1) (#A0[f]) A2)
-     /\(j_invariant m0 n0 (Zpred j1) (#A0[f]) A2)
-       /\(m_invariant m0 A2)
-         /\(n_invariant n0 A2)
-           /\`0 <= (Zpred j1)`
-             /\`(Zs i1) <= N+1`
-               /\(termination (Zs i1) (Zpred j1) m0 n0 (#A0[f]) A2)
-                 /\(permut A2 A).
+Lemma subgoal_3 :
+ forall (m0 n0 i0 j0 i1 j1:Z) (A A0 A1 A2:array Z),
+   array_length A = (N + 1)%Z ->
+   m_invariant m0 A0 /\
+   n_invariant n0 A0 /\ permut A0 A /\ (1 <= m0)%Z /\ (n0 <= N)%Z ->
+   (m0 < n0)%Z ->
+   (0 <= f < Zs N)%Z ->
+   i_invariant m0 n0 i0 (access A0 f) A1 /\
+   j_invariant m0 n0 j0 (access A0 f) A1 /\
+   m_invariant m0 A1 /\
+   n_invariant n0 A1 /\
+   (0 <= j0)%Z /\
+   (i0 <= N + 1)%Z /\
+   termination i0 j0 m0 n0 (access A0 f) A1 /\ permut A1 A ->
+   (i0 <= j0)%Z ->
+   (i_invariant m0 n0 i1 (access A0 f) A1 /\
+    (i0 <= i1)%Z /\
+    (i1 <= n0)%Z /\ termination i1 j0 m0 n0 (access A0 f) A1) /\
+   (access A1 i1 >= access A0 f)%Z ->
+   (j_invariant m0 n0 j1 (access A0 f) A1 /\
+    (j1 <= j0)%Z /\
+    (m0 <= j1)%Z /\ termination i1 j1 m0 n0 (access A0 f) A1) /\
+   (access A0 f >= access A1 j1)%Z ->
+   (access A1 j1 <= access A0 f <= access A1 i1)%Z ->
+   (i1 <= j1)%Z ->
+   exchange A2 A1 i1 j1 ->
+   (access A2 i1 <= access A0 f)%Z ->
+   (access A0 f <= access A2 j1)%Z ->
+   Zwf 0 (N + 2 + Zpred j1 - Zs i1) (N + 2 + j0 - i0) /\
+   i_invariant m0 n0 (Zs i1) (access A0 f) A2 /\
+   j_invariant m0 n0 (Zpred j1) (access A0 f) A2 /\
+   m_invariant m0 A2 /\
+   n_invariant n0 A2 /\
+   (0 <= Zpred j1)%Z /\
+   (Zs i1 <= N + 1)%Z /\
+   termination (Zs i1) (Zpred j1) m0 n0 (access A0 f) A2 /\ permut A2 A.
 Proof.
-Intros m0 n0 i0 j0 i1 j1 A A0 A1 A2 HN Inv_mn Test7 Pre12 Inv_ij Test4 Inv_i 
-  Inv_j Pre10 Test3 Post7 Pre8 Pre7.
-Split.
+intros m0 n0 i0 j0 i1 j1 A A0 A1 A2 HN Inv_mn Test7 Pre12 Inv_ij Test4
+ Inv_i Inv_j Pre10 Test3 Post7 Pre8 Pre7.
+split.
 (* [Zwf] *)
-  Unfold Zwf.
-  Decompose [and] Inv_i. Decompose [and] Inv_j. Unfold Zpred. 
-  Abstract Omega.
-Split.
+  unfold Zwf.
+  decompose [and] Inv_i.
+ decompose [and] Inv_j.
+ unfold Zpred.
+   abstract omega.
+split.
 (* [i_invariant] *)
-  Apply Lemma_8_10 with j:=j1 A':=A1 ; Try Assumption.
-  SameLength A2 A1. Intuition; SameLength A1 A. Omega.
-  Decompose [and] Inv_i. Elim H1. Abstract Omega.
-  Abstract Omega. Abstract Omega.  
-  Decompose [and] Inv_i. Assumption.
-  Decompose [and] Inv_j. Assumption.
-Split.
+  apply Lemma_8_10 with (j := j1) (A' := A1); try assumption.
+  SameLength A2 A1.
+ intuition; SameLength A1 A.
+ omega.
+  decompose [and] Inv_i.
+ elim H1.
+ abstract omega.
+  abstract omega.
+ abstract omega.
+    decompose [and] Inv_i.
+ assumption.
+  decompose [and] Inv_j.
+ assumption.
+split.
 (* [j_invariant] *)
-  Apply Lemma_9_11 with i:=i1 A':=A1 ; Try Assumption.
-  SameLength A2 A1. Intuition; SameLength A1 A. Omega.
-  Decompose [and] Inv_j. Elim H1. Abstract Omega. 
-  Decompose [and] Inv_i. Elim H1. Abstract Omega. 
-  Decompose [and] Inv_mn. Assumption.
-  Decompose [and] Inv_j. Assumption.
-  Decompose [and] Inv_i. Assumption.
-Split.
+  apply Lemma_9_11 with (i := i1) (A' := A1); try assumption.
+  SameLength A2 A1.
+ intuition; SameLength A1 A.
+ omega.
+  decompose [and] Inv_j.
+ elim H1.
+ abstract omega.
+   decompose [and] Inv_i.
+ elim H1.
+ abstract omega.
+   decompose [and] Inv_mn.
+ assumption.
+  decompose [and] Inv_j.
+ assumption.
+  decompose [and] Inv_i.
+ assumption.
+split.
 (* [m_invariant] *)
-  Apply Lemma_12' with i:=i1 j:=j1 A:=A1.
-  Intuition; SameLength A1 A; Omega.
-  Decompose [and] Inv_i. Elim H1. Abstract Omega.
-  Auto with datatypes.
-  Decompose [and] Inv_ij. Assumption.
-Split.
+  apply Lemma_12' with (i := i1) (j := j1) (A := A1).
+  intuition; SameLength A1 A; omega.
+  decompose [and] Inv_i.
+ elim H1.
+ abstract omega.
+  auto with datatypes.
+  decompose [and] Inv_ij.
+ assumption.
+split.
 (* [n_invariant] *)
-  Apply Lemma_13' with i:=i1 j:=j1 A:=A1.
-  Intuition; SameLength A1 A. Omega.
-  Decompose [and] Inv_i. Elim H1. Abstract Omega.
-  Decompose [and] Inv_j. Elim H1. Abstract Omega.
-  Auto with datatypes.
-  Decompose [and] Inv_ij. Assumption.
-Split.
+  apply Lemma_13' with (i := i1) (j := j1) (A := A1).
+  intuition; SameLength A1 A.
+ omega.
+  decompose [and] Inv_i.
+ elim H1.
+ abstract omega.
+  decompose [and] Inv_j.
+ elim H1.
+ abstract omega.
+  auto with datatypes.
+  decompose [and] Inv_ij.
+ assumption.
+split.
 (* [0<=j-1] *)
-  Unfold Zpred. Abstract Omega.
-Split.
+  unfold Zpred.
+ abstract omega.
+split.
 (* [i+1<=N+1] *)
-  Abstract Omega.
-Split.
+  abstract omega.
+split.
 (* [termination] *)
-  Unfold termination. 
-  Left. Unfold Zpred. 
-  Decompose [and] Inv_i. Elim H1. Intros. 
-  Decompose [and] Inv_j. Elim H8. Intros. 
-  Abstract Omega.
+  unfold termination.
+   left.
+ unfold Zpred.
+   decompose [and] Inv_i.
+ elim H1.
+ intros.
+   decompose [and] Inv_j.
+ elim H8.
+ intros.
+   abstract omega.
 (* [permut] *)
-  Decompose [and] Inv_ij. EAuto with datatypes.
-Save.
+  decompose [and] Inv_ij.
+ eauto with datatypes.
+Qed.
 
 
-Lemma subgoal_5 : (m1,n1,i2,j2:Z)(A,A0,A1:(array Z))
-  (m_invariant m1 A0)
-    /\(n_invariant n1 A0)
-    /\(permut A0 A)
-    /\`1 <= m1`/\`n1 <= N` ->
-  `m1 < n1` ->
-  `0 <= f < (Zs N)` ->
-  ((i_invariant m1 n1 i2 (#A0[f]) A1)
-     /\(j_invariant m1 n1 j2 (#A0[f]) A1)
-     /\(m_invariant m1 A1)/\(n_invariant n1 A1)
-     /\`0 <= j2`/\`i2 <= N+1`
-     /\(termination i2 j2 m1 n1 (#A0[f]) A1)
-     /\(permut A1 A))
-    /\`i2 > j2` ->
-  `m1 < i2`/\`j2 < n1` ->
-  `f <= j2` ->
-
-  (Zwf `0` `j2-m1` `n1-m1`)
-   /\(m_invariant m1 A1)
-     /\(n_invariant j2 A1)/\(permut A1 A)/\`1 <= m1`/\`j2 <= N`.
-
-Proof.
-Intros m1 n1 i2 j2 A A0 A1 HH_44 HH_43 HH_41 HH_40 HH_39 HH_37.
-Decompose [and] HH_40.
-Split; [ Idtac | Split; [ Assumption | Split ; 
-           [ Idtac | Split ; [ Assumption | Idtac ]]]].
-Abstract (Unfold Zwf; Elim H; Elim H0; Elim H1; Elim H2; Intros; Omega).
-Apply Lemma_6_a with m:=m1 n:=n1 i:=i2 r:=#A0[f]; Auto.
-Abstract Omega.
-Save.
-
-
-Lemma subgoal_6 : (m1,n1,i2,j2:Z)(A,A0,A1:(array Z))
-  (m_invariant m1 A0)
-    /\(n_invariant n1 A0)
-    /\(permut A0 A)
-    /\`1 <= m1`/\`n1 <= N` ->
-  `m1 < n1` ->
-  `0 <= f < (Zs N)` ->
-  ((i_invariant m1 n1 i2 (#A0[f]) A1)
-     /\(j_invariant m1 n1 j2 (#A0[f]) A1)
-     /\(m_invariant m1 A1)/\(n_invariant n1 A1)
-     /\`0 <= j2`/\`i2 <= N+1`
-     /\(termination i2 j2 m1 n1 (#A0[f]) A1)
-     /\(permut A1 A))
-    /\`i2 > j2` ->
-  `m1 < i2`/\`j2 < n1` ->
-  `f > j2` ->
-  `i2 <= f` -> 
-
-  (Zwf `0` `n1-i2` `n1-m1`)
-   /\(m_invariant i2 A1)
-     /\(n_invariant n1 A1)/\(permut A1 A)/\`1 <= i2`/\`n1 <= N`.
-Proof.
-Intros m1 n1 i2 j2 A A0 A1 HH_44 HH_43 HH_41 HH_40 HH_39 HH_36 HH_33.
-Decompose [and] HH_40.
-Split; [ Idtac | Split ; [Idtac | Split ; [ Assumption | Split ; 
-          [ Assumption | Idtac ]]]].
-Abstract (Unfold Zwf; Elim H; Elim H1; Elim H2; Elim H3; Intros; Omega).
-Apply Lemma_6_b with m:=m1 n:=n1 j:=j2 r:=#A0[f]; Auto.
-Abstract Omega.
-Save.
-
-
-Lemma subgoal_7 : (m1,n1,i2,j2:Z)(A,A0,A1:(array Z))
-  (m_invariant m1 A0)
-    /\(n_invariant n1 A0)/\(permut A0 A)/\`1 <= m1`/\`n1 <= N` ->
-  `m1 < n1` ->
-  `0 <= f < (Zs N)` ->
-  ((i_invariant m1 n1 i2 (#A0[f]) A1)
-     /\(j_invariant m1 n1 j2 (#A0[f]) A1)
-     /\(m_invariant m1 A1)/\(n_invariant n1 A1)
-     /\`0 <= j2`/\`i2 <= N+1`
-     /\(termination i2 j2 m1 n1 (#A0[f]) A1)
-     /\(permut A1 A))
-     /\`i2 > j2` ->
-  `m1 < i2`/\`j2 < n1` ->
-  `f > j2` ->
-  `i2 > f` -> 
-
-  (Zwf `0` `f-f` `n1-m1`)
-   /\(m_invariant f A1)
-     /\(n_invariant f A1)/\(permut A1 A)/\`1 <= f <= N`.
+Lemma subgoal_5 :
+ forall (m1 n1 i2 j2:Z) (A A0 A1:array Z),
+   m_invariant m1 A0 /\
+   n_invariant n1 A0 /\ permut A0 A /\ (1 <= m1)%Z /\ (n1 <= N)%Z ->
+   (m1 < n1)%Z ->
+   (0 <= f < Zs N)%Z ->
+   (i_invariant m1 n1 i2 (access A0 f) A1 /\
+    j_invariant m1 n1 j2 (access A0 f) A1 /\
+    m_invariant m1 A1 /\
+    n_invariant n1 A1 /\
+    (0 <= j2)%Z /\
+    (i2 <= N + 1)%Z /\
+    termination i2 j2 m1 n1 (access A0 f) A1 /\ permut A1 A) /\
+   (i2 > j2)%Z ->
+   (m1 < i2)%Z /\ (j2 < n1)%Z ->
+   (f <= j2)%Z ->
+   Zwf 0 (j2 - m1) (n1 - m1) /\
+   m_invariant m1 A1 /\
+   n_invariant j2 A1 /\ permut A1 A /\ (1 <= m1)%Z /\ (j2 <= N)%Z.
 
 Proof.
-Intros m1 n1 i2 j2 A A0 A1 HH_44 HH_43 HH_41 HH_40 HH_39 HH_36 HH_32.
-Decompose [and] HH_40.
-Split; [ Idtac | Split ; [ Idtac | Split ; [ Idtac | Split ; 
-           [ Assumption | Idtac ]]]].
-Abstract (Unfold Zwf; Elim H; Elim H0; Elim H1; Elim H2; Intros; Omega).
-Apply Lemma_6_c1 with m :=m1 n:=n1 i:=i2 j:=j2 r:=#A0[f]; Auto.
-Abstract Omega.
-Apply Lemma_6_c2 with m :=m1 n:=n1 i:=i2 j:=j2 r:=#A0[f]; Auto.
-Abstract Omega.
-Abstract Omega.
-Save.
+intros m1 n1 i2 j2 A A0 A1 HH_44 HH_43 HH_41 HH_40 HH_39 HH_37.
+decompose [and] HH_40.
+split;
+ [ idtac
+ | split;
+    [ assumption | split; [ idtac | split; [ assumption | idtac ] ] ] ].
+abstract (unfold Zwf; elim H; elim H0; elim H1; elim H2; intros; omega).
+apply Lemma_6_a with (m := m1) (n := n1) (i := i2) (r := access A0 f);
+ auto.
+abstract omega.
+Qed.
+
+
+Lemma subgoal_6 :
+ forall (m1 n1 i2 j2:Z) (A A0 A1:array Z),
+   m_invariant m1 A0 /\
+   n_invariant n1 A0 /\ permut A0 A /\ (1 <= m1)%Z /\ (n1 <= N)%Z ->
+   (m1 < n1)%Z ->
+   (0 <= f < Zs N)%Z ->
+   (i_invariant m1 n1 i2 (access A0 f) A1 /\
+    j_invariant m1 n1 j2 (access A0 f) A1 /\
+    m_invariant m1 A1 /\
+    n_invariant n1 A1 /\
+    (0 <= j2)%Z /\
+    (i2 <= N + 1)%Z /\
+    termination i2 j2 m1 n1 (access A0 f) A1 /\ permut A1 A) /\
+   (i2 > j2)%Z ->
+   (m1 < i2)%Z /\ (j2 < n1)%Z ->
+   (f > j2)%Z ->
+   (i2 <= f)%Z ->
+   Zwf 0 (n1 - i2) (n1 - m1) /\
+   m_invariant i2 A1 /\
+   n_invariant n1 A1 /\ permut A1 A /\ (1 <= i2)%Z /\ (n1 <= N)%Z.
+Proof.
+intros m1 n1 i2 j2 A A0 A1 HH_44 HH_43 HH_41 HH_40 HH_39 HH_36 HH_33.
+decompose [and] HH_40.
+split;
+ [ idtac
+ | split;
+    [ idtac | split; [ assumption | split; [ assumption | idtac ] ] ] ].
+abstract (unfold Zwf; elim H; elim H1; elim H2; elim H3; intros; omega).
+apply Lemma_6_b with (m := m1) (n := n1) (j := j2) (r := access A0 f);
+ auto.
+abstract omega.
+Qed.
+
+
+Lemma subgoal_7 :
+ forall (m1 n1 i2 j2:Z) (A A0 A1:array Z),
+   m_invariant m1 A0 /\
+   n_invariant n1 A0 /\ permut A0 A /\ (1 <= m1)%Z /\ (n1 <= N)%Z ->
+   (m1 < n1)%Z ->
+   (0 <= f < Zs N)%Z ->
+   (i_invariant m1 n1 i2 (access A0 f) A1 /\
+    j_invariant m1 n1 j2 (access A0 f) A1 /\
+    m_invariant m1 A1 /\
+    n_invariant n1 A1 /\
+    (0 <= j2)%Z /\
+    (i2 <= N + 1)%Z /\
+    termination i2 j2 m1 n1 (access A0 f) A1 /\ permut A1 A) /\
+   (i2 > j2)%Z ->
+   (m1 < i2)%Z /\ (j2 < n1)%Z ->
+   (f > j2)%Z ->
+   (i2 > f)%Z ->
+   Zwf 0 (f - f) (n1 - m1) /\
+   m_invariant f A1 /\
+   n_invariant f A1 /\ permut A1 A /\ (1 <= f <= N)%Z.
+
+Proof.
+intros m1 n1 i2 j2 A A0 A1 HH_44 HH_43 HH_41 HH_40 HH_39 HH_36 HH_32.
+decompose [and] HH_40.
+split;
+ [ idtac
+ | split; [ idtac | split; [ idtac | split; [ assumption | idtac ] ] ] ].
+abstract (unfold Zwf; elim H; elim H0; elim H1; elim H2; intros; omega).
+apply Lemma_6_c1 with
+ (m := m1) (n := n1) (i := i2) (j := j2) (r := access A0 f); auto.
+abstract omega.
+apply Lemma_6_c2 with
+ (m := m1) (n := n1) (i := i2) (j := j2) (r := access A0 f); auto.
+abstract omega.
+abstract omega.
+Qed.
