examples/linked-lists/length_why.v
@@ -1,137 +1,94 @@
+(* Load Programs. *)
+Require Import Why.
 
-Require Why.
+Require Import LinkedLists.
 
-Require LinkedLists.
-
-(* Why obligation from file "length.mlw", characters 1039-1200 *)
-Lemma length_po_1 : 
-  (p0: pointer)
-  (Ltl: pointer_store)
-  (Pre4: (is_list Ltl p0))
-  (p: pointer)
-  (Post8: p = p0)
-  (n: Z)
-  (Post7: n = `0`)
-  (well_founded ll_order).
+(* Why obligation from file , characters 1039-1200 *)
+Lemma length_po_1 :
+ forall (p0:pointer) (Ltl:pointer_store) (Pre4:is_list Ltl p0)
+   (p:pointer) (Post8:p = p0) (n:Z) (Post7:n = 0%Z),
+   well_founded ll_order.
 Proof.
-Auto.
-Save.
+auto.
+Qed.
 
-(* Why obligation from file "length.mlw", characters 1045-1061 *)
-Lemma length_po_2 : 
-  (p0: pointer)
-  (Ltl: pointer_store)
-  (Pre4: (is_list Ltl p0))
-  (p: pointer)
-  (Post8: p = p0)
-  (n: Z)
-  (Post7: n = `0`)
-  (Variant1: StorePointerPair)
-  (p2: pointer)
-  (Pre3: Variant1 = (store_pointer_pair Ltl p2))
-  (Pre2: (is_list Ltl p2))
-  (Test2: p2 = null)
-  (result0: bool)
-  (Post3: result0 = false)
-  (if result0 then p2 = null /\ true = false \/ ~(p2 = null) /\ true = true
-   else p2 = null /\ false = false \/ ~(p2 = null) /\ false = true).
+(* Why obligation from file , characters 1061-1061 *)
+Lemma length_po_2 :
+ forall (p0:pointer) (Ltl:pointer_store) (Pre4:is_list Ltl p0)
+   (p:pointer) (Post8:p = p0) (n:Z) (Post7:n = 0%Z)
+   (Variant1:StorePointerPair) (p2:pointer)
+   (Pre3:Variant1 = store_pointer_pair Ltl p2) (Pre2:is_list Ltl p2)
+   (Test2:p2 = null) (result0:bool) (Post3:result0 = false),
+   if result0
+   then p2 = null /\ true = false \/ p2 <> null /\ true = true
+   else p2 = null /\ false = false \/ p2 <> null /\ false = true.
 Proof.
-Destruct result0; Intuition.
-Save.
+olddestruct result0; intuition.
+Qed.
 
-(* Why obligation from file "length.mlw", characters 1045-1061 *)
-Lemma length_po_3 : 
-  (p0: pointer)
-  (Ltl: pointer_store)
-  (Pre4: (is_list Ltl p0))
-  (p: pointer)
-  (Post8: p = p0)
-  (n: Z)
-  (Post7: n = `0`)
-  (Variant1: StorePointerPair)
-  (p2: pointer)
-  (Pre3: Variant1 = (store_pointer_pair Ltl p2))
-  (Pre2: (is_list Ltl p2))
-  (Test1: ~(p2 = null))
-  (result0: bool)
-  (Post4: result0 = true)
-  (if result0 then p2 = null /\ true = false \/ ~(p2 = null) /\ true = true
-   else p2 = null /\ false = false \/ ~(p2 = null) /\ false = true).
+(* Why obligation from file , characters 1061-1061 *)
+Lemma length_po_3 :
+ forall (p0:pointer) (Ltl:pointer_store) (Pre4:is_list Ltl p0)
+   (p:pointer) (Post8:p = p0) (n:Z) (Post7:n = 0%Z)
+   (Variant1:StorePointerPair) (p2:pointer)
+   (Pre3:Variant1 = store_pointer_pair Ltl p2) (Pre2:is_list Ltl p2)
+   (Test1:p2 <> null) (result0:bool) (Post4:result0 = true),
+   if result0
+   then p2 = null /\ true = false \/ p2 <> null /\ true = true
+   else p2 = null /\ false = false \/ p2 <> null /\ false = true.
 Proof.
-Destruct result0; Intuition.
-Save.
+olddestruct result0; intuition.
+Qed.
 
-(* Why obligation from file "length.mlw", characters 1039-1200 *)
-Lemma length_po_4 : 
-  (p0: pointer)
-  (Ltl: pointer_store)
-  (Pre4: (is_list Ltl p0))
-  (p: pointer)
-  (Post8: p = p0)
-  (n: Z)
-  (Post7: n = `0`)
-  (Variant1: StorePointerPair)
-  (n1: Z)
-  (p2: pointer)
-  (Pre3: Variant1 = (store_pointer_pair Ltl p2))
-  (Pre2: (is_list Ltl p2))
-  (Test4: p2 = null /\ true = false \/ ~(p2 = null) /\ true = true)
-  (n2: Z)
-  (Post1: n2 = `n1 + 1`)
-  (p3: pointer)
-  (Post2: p3 = (pget Ltl p2))
-  (is_list Ltl p3) /\
-  (ll_order (store_pointer_pair Ltl p3) (store_pointer_pair Ltl p2)).
+(* Why obligation from file , characters 1157-1193 *)
+Lemma length_po_4 :
+ forall (p0:pointer) (Ltl:pointer_store) (Pre4:is_list Ltl p0)
+   (p:pointer) (Post8:p = p0) (n:Z) (Post7:n = 0%Z)
+   (Variant1:StorePointerPair) (n1:Z) (p2:pointer)
+   (Pre3:Variant1 = store_pointer_pair Ltl p2) (Pre2:is_list Ltl p2)
+   (Test4:p2 = null /\ true = false \/ p2 <> null /\ true = true)
+   (n2:Z) (Post1:n2 = (n1 + 1)%Z) (p3:pointer)
+   (Post2:p3 = pget Ltl p2),
+   is_list Ltl p3 /\
+   ll_order (store_pointer_pair Ltl p3) (store_pointer_pair Ltl p2).
 Proof.
-Intuition.
-Discriminate H1.
-Discriminate H1.
-Inversion Pre2.
-Rewrite H in H0; Intuition.
-Case (eq_null_dec p3); Intro.
-Clear Post2; Subst p3; Auto.
-Subst p3; Auto.
-Unfold store_pointer_pair ll_order.
-Generalize (is_list_llist ? ? Pre2).
-Intros (l, Hl).
-Inversion Hl; Intuition.
-Exists l0; Exists l; Subst; Intuition.
-Rewrite <- H4; Simpl; Omega.
-Save.
+intuition.
+discriminate H1.
+discriminate H1.
+inversion Pre2.
+rewrite H in H0; intuition.
+case (eq_null_dec p3); intro.
+clear Post2; subst p3; auto.
+subst p3; auto.
+unfold store_pointer_pair, ll_order.
+generalize (is_list_llist _ _ Pre2).
+intros [l Hl].
+inversion Hl; intuition.
+exists l0; exists l; subst; intuition.
+rewrite <- H4; simpl; omega.
+Qed.
 
-(* Why obligation from file "length.mlw", characters 1039-1200 *)
-Lemma length_po_5 : 
-  (p0: pointer)
-  (Ltl: pointer_store)
-  (Pre4: (is_list Ltl p0))
-  (p: pointer)
-  (Post8: p = p0)
-  (n: Z)
-  (Post7: n = `0`)
-  (Variant1: StorePointerPair)
-  (p2: pointer)
-  (Pre3: Variant1 = (store_pointer_pair Ltl p2))
-  (Pre2: (is_list Ltl p2))
-  (Test4: p2 = null /\ true = false \/ ~(p2 = null) /\ true = true)
-  (p3: pointer)
-  (Post10: (is_list Ltl p3) /\
-           (ll_order (store_pointer_pair Ltl p3) (store_pointer_pair Ltl p2)))
-  (ll_order (store_pointer_pair Ltl p3) Variant1).
+(* Why obligation from file , characters 1039-1200 *)
+Lemma length_po_5 :
+ forall (p0:pointer) (Ltl:pointer_store) (Pre4:is_list Ltl p0)
+   (p:pointer) (Post8:p = p0) (n:Z) (Post7:n = 0%Z)
+   (Variant1:StorePointerPair) (p2:pointer)
+   (Pre3:Variant1 = store_pointer_pair Ltl p2) (Pre2:is_list Ltl p2)
+   (Test4:p2 = null /\ true = false \/ p2 <> null /\ true = true)
+   (p3:pointer)
+   (Post10:is_list Ltl p3 /\
+           ll_order (store_pointer_pair Ltl p3)
+             (store_pointer_pair Ltl p2)),
+   ll_order (store_pointer_pair Ltl p3) Variant1.
 Proof.
-Intros; Rewrite Pre3; Intuition.
-Save.
+intros; rewrite Pre3; intuition.
+Qed.
 
-(* Why obligation from file "length.mlw", characters 1081-1096 *)
-Lemma length_po_6 : 
-  (p0: pointer)
-  (Ltl: pointer_store)
-  (Pre4: (is_list Ltl p0))
-  (p: pointer)
-  (Post8: p = p0)
-  (n: Z)
-  (Post7: n = `0`)
-  (is_list Ltl p).
+(* Why obligation from file , characters 1081-1096 *)
+Lemma length_po_6 :
+ forall (p0:pointer) (Ltl:pointer_store) (Pre4:is_list Ltl p0)
+   (p:pointer) (Post8:p = p0) (n:Z) (Post7:n = 0%Z), is_list Ltl p.
 Proof.
-Intros; Subst p; Intuition.
-Save.
+intros; subst p; intuition.
+Qed.
 
