examples/linked-lists/rev_why.v
@@ -1,189 +1,156 @@
-
-Require Why.
+(* Load Programs. *)
+Require Import Why.
 
 Require Export LinkedLists.
 
-(* Why obligation from file "rev.mlw", characters 1173-1631 *)
-Lemma rev_po_1 : 
-  (p0: pointer)
-  (Ltl: pointer_store)
-  (Pre4: (is_list Ltl p0))
-  (p: pointer)
-  (Post8: p = p0)
-  (r: pointer)
-  (Post7: r = p)
-  (p2: pointer)
-  (Post1: p2 = null)
-  (well_founded ll_order).
+(* Why obligation from file , characters 1173-1631 *)
+Lemma rev_po_1 :
+ forall (p0:pointer) (Ltl:pointer_store) (Pre4:is_list Ltl p0)
+   (p:pointer) (Post8:p = p0) (r:pointer) (Post7:r = p) (p2:pointer)
+   (Post1:p2 = null), well_founded ll_order.
 Proof.
-Auto.
-Save.
+auto.
+Qed.
 
 (* should go in PolyList *)
-Lemma app_rev_cons : 
-  (A:Set)(l1,l2:(list A))(x:A)
-  (app (rev l1) (cons x l2)) = (app (rev (cons x l1)) l2).
+Lemma app_rev_cons :
+ forall (A:Set) (l1 l2:list A) (x:A),
+   app (rev l1) (cons x l2) = app (rev (cons x l1)) l2.
 Proof.
-Intros; Simpl.
-Rewrite app_ass; Auto.
-Save.
+intros; simpl.
+rewrite app_ass; auto.
+Qed.
 
 
-(* Why obligation from file "rev.mlw", characters 1534-1622 *)
-Lemma rev_po_2 : 
-  (p0: pointer)
-  (Ltl: pointer_store)
-  (Pre4: (is_list Ltl p0))
-  (p: pointer)
-  (Post8: p = p0)
-  (r: pointer)
-  (Post7: r = p)
-  (p2: pointer)
-  (Post1: p2 = null)
-  (Variant1: StorePointerPair)
-  (Ltl0: pointer_store)
-  (p3: pointer)
-  (r1: pointer)
-  (Pre3: Variant1 = (store_pointer_pair Ltl0 r1))
-  (Pre2: (EX lp:plist |
-          (EX lr:plist | (llist Ltl0 p3 lp) /\ (llist Ltl0 r1 lr) /\
-           (disjoint lp lr) /\
-           ((l:plist) ((llist Ltl p0 l) -> (app (rev lr) lp) = (rev l))))))
-  (Test2: ~(r1 = null))
-  (q: pointer)
-  (Post5: q = r1)
-  (r2: pointer)
-  (Post2: r2 = (pget Ltl0 r1))
-  (Ltl1: pointer_store)
-  (Post3: Ltl1 = (pset Ltl0 q p3))
-  (p4: pointer)
-  (Post4: p4 = q)
-  (EX lp:plist |
-   (EX lr:plist | (llist Ltl1 p4 lp) /\ (llist Ltl1 r2 lr) /\
-    (disjoint lp lr) /\
-    ((l:plist) ((llist Ltl p0 l) -> (app (rev lr) lp) = (rev l))))) /\
-  (ll_order (store_pointer_pair Ltl1 r2) (store_pointer_pair Ltl0 r1)).
+(* Why obligation from file , characters 1534-1622 *)
+Lemma rev_po_2 :
+ forall (p0:pointer) (Ltl:pointer_store) (Pre4:is_list Ltl p0)
+   (p:pointer) (Post8:p = p0) (r:pointer) (Post7:r = p) (p2:pointer)
+   (Post1:p2 = null) (Variant1:StorePointerPair) (Ltl0:pointer_store)
+   (p3 r1:pointer) (Pre3:Variant1 = store_pointer_pair Ltl0 r1)
+   (Pre2: EX lp : plist
+         | ( EX lr : plist
+            | llist Ltl0 p3 lp /\
+              llist Ltl0 r1 lr /\
+              disjoint lp lr /\
+              (forall l:plist,
+                 llist Ltl p0 l -> app (rev lr) lp = rev l)))
+   (Test2:r1 <> null) (q:pointer) (Post5:q = r1) (r2:pointer)
+   (Post2:r2 = pget Ltl0 r1) (Ltl1:pointer_store)
+   (Post3:Ltl1 = pset Ltl0 q p3) (p4:pointer) (Post4:p4 = q),
+   ( EX lp : plist
+    | ( EX lr : plist
+       | llist Ltl1 p4 lp /\
+         llist Ltl1 r2 lr /\
+         disjoint lp lr /\
+         (forall l:plist, llist Ltl p0 l -> app (rev lr) lp = rev l))) /\
+   ll_order (store_pointer_pair Ltl1 r2) (store_pointer_pair Ltl0 r1).
 Proof.
-Intuition.
-Elim Pre2; Clear Pre2; Intuition.
-Elim H; Clear H; Intuition.
-Subst.
-Inversion H.
-Absurd r1=null; Intuition.
-Exists (cons r1 x); Exists l; Subst; Intuition.
-Unfold llist; Apply Path_cons; Intuition.
-Rewrite PointerStore.get_set_same; Auto.
-Apply llist_pset_same; Auto.
-Unfold disjoint in H1; Intuition.
-Apply (H7 r1); Auto.
-Rewrite <- H6; Auto with *.
-Apply llist_pset_same; Auto.
-Apply llist_not_starting with Ltl0; Auto.
-Apply disjoint_cons.
-Rewrite H6; Auto.
-Apply llist_not_starting with Ltl0; Auto.
-Rewrite app_rev_cons.
-Rewrite H6; Apply H3; Auto.
-Unfold ll_order store_pointer_pair.
-Elim Pre2; Clear Pre2; Intuition.
-Elim H; Clear H; Intuition.
-Subst.
-Inversion H; Intuition.
-Exists l; Exists x0; Intuition.
-Apply llist_pset_same; Auto.
-Apply llist_not_starting with Ltl0; Auto.
-Rewrite <- H6; Simpl; Omega.
-Save.
+intuition.
+elim Pre2; clear Pre2; intuition.
+elim H; clear H; intuition.
+subst.
+inversion H.
+absurd (r1 = null); intuition.
+exists (cons r1 x); exists l; subst; intuition.
+unfold llist; apply Path_cons; intuition.
+ rewrite PointerStore.get_set_same; auto.
+apply llist_pset_same; auto.
+unfold disjoint in H1; intuition.
+apply (H7 r1); auto.
+rewrite <- H6; auto with *.
+apply llist_pset_same; auto.
+apply llist_not_starting with Ltl0; auto.
+apply disjoint_cons.
+rewrite H6; auto.
+apply llist_not_starting with Ltl0; auto.
+rewrite app_rev_cons.
+rewrite H6; apply H3; auto.
+unfold ll_order, store_pointer_pair.
+elim Pre2; clear Pre2; intuition.
+elim H; clear H; intuition.
+subst.
+inversion H; intuition.
+exists l; exists x0; intuition.
+apply llist_pset_same; auto.
+apply llist_not_starting with Ltl0; auto.
+rewrite <- H6; simpl; omega.
+Qed.
 
-(* Why obligation from file "rev.mlw", characters 1173-1631 *)
-Lemma rev_po_3 : 
-  (p0: pointer)
-  (Ltl: pointer_store)
-  (Pre4: (is_list Ltl p0))
-  (p: pointer)
-  (Post8: p = p0)
-  (r: pointer)
-  (Post7: r = p)
-  (p2: pointer)
-  (Post1: p2 = null)
-  (Variant1: StorePointerPair)
-  (Ltl0: pointer_store)
-  (p3: pointer)
-  (r1: pointer)
-  (Pre3: Variant1 = (store_pointer_pair Ltl0 r1))
-  (Pre2: (EX lp:plist |
-          (EX lr:plist | (llist Ltl0 p3 lp) /\ (llist Ltl0 r1 lr) /\
-           (disjoint lp lr) /\
-           ((l:plist) ((llist Ltl p0 l) -> (app (rev lr) lp) = (rev l))))))
-  (Test2: ~(r1 = null))
-  (Ltl1: pointer_store)
-  (p4: pointer)
-  (r2: pointer)
-  (Post9: (EX lp:plist |
-           (EX lr:plist | (llist Ltl1 p4 lp) /\ (llist Ltl1 r2 lr) /\
-            (disjoint lp lr) /\
-            ((l:plist) ((llist Ltl p0 l) -> (app (rev lr) lp) = (rev l))))) /\
-          (ll_order (store_pointer_pair Ltl1 r2) (store_pointer_pair Ltl0 r1)))
-  (ll_order (store_pointer_pair Ltl1 r2) Variant1).
+(* Why obligation from file , characters 1173-1631 *)
+Lemma rev_po_3 :
+ forall (p0:pointer) (Ltl:pointer_store) (Pre4:is_list Ltl p0)
+   (p:pointer) (Post8:p = p0) (r:pointer) (Post7:r = p) (p2:pointer)
+   (Post1:p2 = null) (Variant1:StorePointerPair) (Ltl0:pointer_store)
+   (p3 r1:pointer) (Pre3:Variant1 = store_pointer_pair Ltl0 r1)
+   (Pre2: EX lp : plist
+         | ( EX lr : plist
+            | llist Ltl0 p3 lp /\
+              llist Ltl0 r1 lr /\
+              disjoint lp lr /\
+              (forall l:plist,
+                 llist Ltl p0 l -> app (rev lr) lp = rev l)))
+   (Test2:r1 <> null) (Ltl1:pointer_store) (p4 r2:pointer)
+   (Post9:( EX lp : plist
+           | ( EX lr : plist
+              | llist Ltl1 p4 lp /\
+                llist Ltl1 r2 lr /\
+                disjoint lp lr /\
+                (forall l:plist,
+                   llist Ltl p0 l -> app (rev lr) lp = rev l))) /\
+          ll_order (store_pointer_pair Ltl1 r2)
+            (store_pointer_pair Ltl0 r1)),
+   ll_order (store_pointer_pair Ltl1 r2) Variant1.
 Proof.
-Intros; Subst Variant1; Intuition.
-Save.
+intros; subst Variant1; intuition.
+Qed.
 
-(* Why obligation from file "rev.mlw", characters 1222-1445 *)
-Lemma rev_po_4 : 
-  (p0: pointer)
-  (Ltl: pointer_store)
-  (Pre4: (is_list Ltl p0))
-  (p: pointer)
-  (Post8: p = p0)
-  (r: pointer)
-  (Post7: r = p)
-  (p2: pointer)
-  (Post1: p2 = null)
-  (EX lp:plist |
-   (EX lr:plist | (llist Ltl p2 lp) /\ (llist Ltl r lr) /\
-    (disjoint lp lr) /\
-    ((l:plist) ((llist Ltl p0 l) -> (app (rev lr) lp) = (rev l))))).
+(* Why obligation from file , characters 1222-1445 *)
+Lemma rev_po_4 :
+ forall (p0:pointer) (Ltl:pointer_store) (Pre4:is_list Ltl p0)
+   (p:pointer) (Post8:p = p0) (r:pointer) (Post7:r = p) (p2:pointer)
+   (Post1:p2 = null),
+    EX lp : plist
+   | ( EX lr : plist
+      | llist Ltl p2 lp /\
+        llist Ltl r lr /\
+        disjoint lp lr /\
+        (forall l:plist, llist Ltl p0 l -> app (rev lr) lp = rev l)).
 Proof.
-Intros; Subst.
-Exists (nil pointer).
-Elim (is_list_llist Ltl p0 Pre4); Intros l Hl; Exists l.
-Intuition.
-Rewrite (llist_function ? ? ? ? Hl H).
-Intuition.
-Save.
+intros; subst.
+exists (nil (A:=pointer)).
+elim (is_list_llist Ltl p0 Pre4); intros l Hl; exists l.
+intuition.
+rewrite (llist_function _ _ _ _ Hl H).
+intuition.
+Qed.
 
-(* Why obligation from file "rev.mlw", characters 1637-1639 *)
-Lemma rev_po_5 : 
-  (p0: pointer)
-  (Ltl: pointer_store)
-  (Pre4: (is_list Ltl p0))
-  (p: pointer)
-  (Post8: p = p0)
-  (r: pointer)
-  (Post7: r = p)
-  (p2: pointer)
-  (Post1: p2 = null)
-  (Ltl0: pointer_store)
-  (p3: pointer)
-  (r1: pointer)
-  (Post6: (EX lp:plist |
-           (EX lr:plist | (llist Ltl0 p3 lp) /\ (llist Ltl0 r1 lr) /\
-            (disjoint lp lr) /\
-            ((l:plist) ((llist Ltl p0 l) -> (app (rev lr) lp) = (rev l))))) /\
-          r1 = null)
-  (EX l:plist | (llist Ltl0 p3 l) /\
-   ((l0:plist) ((llist Ltl p0 l0) -> l = (rev l0)))).
+(* Why obligation from file , characters 1637-1639 *)
+Lemma rev_po_5 :
+ forall (p0:pointer) (Ltl:pointer_store) (Pre4:is_list Ltl p0)
+   (p:pointer) (Post8:p = p0) (r:pointer) (Post7:r = p) (p2:pointer)
+   (Post1:p2 = null) (Ltl0:pointer_store) (p3 r1:pointer)
+   (Post6:( EX lp : plist
+           | ( EX lr : plist
+              | llist Ltl0 p3 lp /\
+                llist Ltl0 r1 lr /\
+                disjoint lp lr /\
+                (forall l:plist,
+                   llist Ltl p0 l -> app (rev lr) lp = rev l))) /\
+          r1 = null),
+    EX l : plist
+   | llist Ltl0 p3 l /\
+     (forall l0:plist, llist Ltl p0 l0 -> l = rev l0).
 Proof.
-Intuition.
-Elim H; Clear H; Intros lp H; Elim H; Clear H; Intro lr; Intuition.
-Exists lp; Intuition.
-Subst r1.
-Inversion H.
-Rewrite <- (H4 l0); Auto.
-Rewrite <- H5; Trivial.
-Subst.
-Inversion H0.
-Save.
+intuition.
+elim H; clear H; intros lp H; elim H; clear H; intro lr; intuition.
+exists lp; intuition.
+subst r1.
+inversion H.
+rewrite <- (H4 l0); auto.
+rewrite <- H5; trivial.
+subst.
+inversion H0.
+Qed.
 
 
