examples/quicksort/Quicksort.v
@@ -1,4 +1,4 @@
-(**************************************************************************)
+(* Load Programs. *)(**************************************************************************)
 (*                                                                        *)
 (* Proof of the Quicksort Algorithm.                                      *)
 (*                                                                        *)
@@ -7,10 +7,10 @@
 (*                                                                        *)
 (**************************************************************************)
 
-Require Why.
-Require Partition.
+Require Import Why.
+Require Import Partition.
 
-Require Omega.
+Require Import Omega.
 
 (* Here we prove the main lemma of quicksort:
  *
@@ -27,75 +27,89 @@ Require Omega.
  *)
 
 Lemma quicksort_lemma :
-  (t0,t1,t2,t3:(array Z))
-  (g,d,p:Z) `0 <= g` -> `g < d` -> `d < (array_length t0)` -> `g <= p <= d`
-    -> (partition_p t1 g d p) -> (sub_permut g d t1 t0)
-     -> (sorted_array t2 g (Zpred p)) -> (sub_permut g (Zpred p) t2 t1)
-       -> (sorted_array t3 (Zs p) d) -> (sub_permut(Zs p) d t3 t2 )
-         -> (sorted_array t3 g d) /\ (sub_permut g d t3 t0).
+ forall (t0 t1 t2 t3:array Z) (g d p:Z),
+   (0 <= g)%Z ->
+   (g < d)%Z ->
+   (d < array_length t0)%Z ->
+   (g <= p <= d)%Z ->
+   partition_p t1 g d p ->
+   sub_permut g d t1 t0 ->
+   sorted_array t2 g (Zpred p) ->
+   sub_permut g (Zpred p) t2 t1 ->
+   sorted_array t3 (Zs p) d ->
+   sub_permut (Zs p) d t3 t2 ->
+   sorted_array t3 g d /\ sub_permut g d t3 t0.
 Proof.
-Intros t0 t1 t2 t3 g d p H1 H2 H3 H4
-  piv_t1 perm_t1 sort_t2 perm_t2 sort_t3 perm_t3.
-Generalize (sub_permut_length perm_t1); Intro HL1. 
-Generalize (sub_permut_length perm_t2); Intro HL2. 
-Generalize (sub_permut_length perm_t3); Intro HL3. 
-Rewrite <- HL1 in H3.
-Generalize
-  (partition_p_permut_left H1 H2 H3 H4 piv_t1 (sub_permut_sym perm_t2)).
-  Intro piv_t2.
-Rewrite <- HL2 in H3.
-Generalize 
-  (partition_p_permut_right H1 H2 H3 H4 piv_t2 (sub_permut_sym perm_t3)).
-  Intro piv_t3.
-Generalize (sub_permut_is_permut perm_t1); Intro.
-  Elim (sub_permut_id perm_t1); Intros.
-Generalize (sub_permut_is_permut perm_t2); Intro.
-  Elim (sub_permut_id perm_t2); Intros.
-Generalize (sub_permut_is_permut perm_t3); Intro.
-  Elim (sub_permut_id perm_t3); Intros.
-Split.
+intros t0 t1 t2 t3 g d p H1 H2 H3 H4 piv_t1 perm_t1 sort_t2 perm_t2
+ sort_t3 perm_t3.
+generalize (sub_permut_length perm_t1); intro HL1.
+ generalize (sub_permut_length perm_t2); intro HL2.
+ generalize (sub_permut_length perm_t3); intro HL3.
+ rewrite <- HL1 in H3.
+generalize
+ (partition_p_permut_left H1 H2 H3 H4 piv_t1 (sub_permut_sym perm_t2)).
+  intro piv_t2.
+rewrite <- HL2 in H3.
+generalize
+ (partition_p_permut_right H1 H2 H3 H4 piv_t2 (sub_permut_sym perm_t3)).
+  intro piv_t3.
+generalize (sub_permut_is_permut perm_t1); intro.
+  elim (sub_permut_id perm_t1); intros.
+generalize (sub_permut_is_permut perm_t2); intro.
+  elim (sub_permut_id perm_t2); intros.
+generalize (sub_permut_is_permut perm_t3); intro.
+  elim (sub_permut_id perm_t3); intros.
+split.
 (* sorted_array *)
-Unfold sorted_array. Intros.
-Elim (Z_lt_ge_dec x `p-1`); Intros.
+unfold sorted_array.
+ intros.
+elim (Z_lt_ge_dec x (p - 1)); intros.
 (* x < p-1 *)
-Unfold array_id in H10.
-Rewrite (H10 x); Try Omega. Rewrite (H10 `x+1`); Try Omega.
-Unfold sorted_array in sort_t2.
-Apply sort_t2; Unfold Zpred; Omega.
-Elim (Z_lt_ge_dec x p); Intros.
+unfold array_id in H10.
+rewrite (H10 x); try omega.
+ rewrite (H10 (x + 1)%Z); try omega.
+unfold sorted_array in sort_t2.
+apply sort_t2; unfold Zpred; omega.
+elim (Z_lt_ge_dec x p); intros.
 (* x = p-1 *)
-Elim piv_t3; Intros.
-Elim H17; Intros.
-Cut `x+1=p`. Intro Heq. Rewrite Heq.
-Apply H19; Omega.
-Omega.
-Elim (Z_lt_ge_dec x `p+1`); Intros.
+elim piv_t3; intros.
+elim H17; intros.
+cut ((x + 1)%Z = p).
+ intro Heq.
+ rewrite Heq.
+apply H19; omega.
+omega.
+elim (Z_lt_ge_dec x (p + 1)); intros.
 (* x = p *)
-Elim piv_t3; Intros.
-Elim H18; Intros.
-Cut `x=p`. Intro Heq. Rewrite Heq.
-Apply H19; Omega.
-Omega.
+elim piv_t3; intros.
+elim H18; intros.
+cut (x = p).
+ intro Heq.
+ rewrite Heq.
+apply H19; omega.
+omega.
 (* x > p *)
-Unfold sorted_array in sort_t3.
-Apply sort_t3; Unfold Zs; Omega.
+unfold sorted_array in sort_t3.
+apply sort_t3; unfold Zs; omega.
 
 (* sub_permut *)
-Apply sub_permut_trans with t':=t2.
-Elim (Z_le_gt_dec (Zs p) d); Intro.
-Apply sub_permut_extension with g:=(Zs p) d:=d; Try Omega.
-Assumption.
-Apply sub_permut_void with g:=(Zs p) d:=d; Try Omega.
-Assumption.
-Apply sub_permut_trans with t':=t1.
-Elim (Z_le_gt_dec g (Zpred p)); Intro.
-Apply sub_permut_extension with g:=g d:=(Zpred p); Try (Unfold Zpred;Omega).
-Assumption.
-Apply sub_permut_void with g:=g d:=(Zpred p); Try (Unfold Zpred;Omega).
-Omega.
-Assumption.
-Assumption.
-Save.
+apply sub_permut_trans with (t' := t2).
+elim (Z_le_gt_dec (Zs p) d); intro.
+apply sub_permut_extension with (g := Zs p) (d := d); try omega.
+assumption.
+apply sub_permut_void with (g := Zs p) (d := d); try omega.
+assumption.
+apply sub_permut_trans with (t' := t1).
+elim (Z_le_gt_dec g (Zpred p)); intro.
+apply sub_permut_extension with (g := g) (d := Zpred p);
+ try (unfold Zpred; omega).
+assumption.
+apply sub_permut_void with (g := g) (d := Zpred p);
+ try (unfold Zpred; omega).
+omega.
+assumption.
+assumption.
+Qed.
 
 
 (* The trivial case, when the segment of the array contains at most
@@ -103,16 +117,17 @@ Save.
  *)
 
 Lemma quicksort_trivial :
-  (t:(array Z))
-  (g,d:Z) `0 <= g` -> `g >= d` -> `d < (array_length t)`
-    -> (sorted_array t g d) /\ (sub_permut g d t t).
+ forall (t:array Z) (g d:Z),
+   (0 <= g)%Z ->
+   (g >= d)%Z ->
+   (d < array_length t)%Z -> sorted_array t g d /\ sub_permut g d t t.
 Proof.
-Intros t g d H1 H2 H3.
-Split.
-Unfold sorted_array.
-Intros.
-(Absurd `x < d`; Omega).
-Auto with datatypes.
-Save.
+intros t g d H1 H2 H3.
+split.
+unfold sorted_array.
+intros.
+absurd (x < d)%Z; omega.
+auto with datatypes.
+Qed.
 
     
