examples/sqrt/sqrt_why.v
@@ -1,4 +1,4 @@
-(********************************************************************
+(* Load Programs. *)(********************************************************************
 
   A simple algorithm for computing the square root of a non-negative
   integer.
@@ -13,361 +13,341 @@
    It can be modified; only the generated parts will be overwritten. *)
 
 
-Require ZArith.
-Require Zcomplements.
-Require ZArithRing.
-Require Zdiv.
-Require Omega.
-Require Why.
+Require Import ZArith.
+Require Import Zcomplements.
+Require Import ZArithRing.
+Require Import Zdiv.
+Require Import Omega.
+Require Import Why.
 
 (* some basic arithmetic lemmas *)
 
-Lemma sqr_gt:(x,y:Z)`x > y`->`y > 0`->`x*x > y*y`.
+Lemma sqr_gt :
+ forall x y:Z, (x > y)%Z -> (y > 0)%Z -> (x * x > y * y)%Z.
 Proof.
-Intros.
-Assert `x*y > y*y`.
-Apply Zgt_Zmult_right; Omega.
-Assert `x*x > x*y`.
-Apply Zgt_Zmult_left; Omega.
-Omega.
-Save.
+intros.
+assert (x * y > y * y)%Z.
+apply Zgt_Zmult_right; omega.
+assert (x * x > x * y)%Z.
+apply Zgt_Zmult_left; omega.
+omega.
+Qed.
 
-Lemma Z_mod_same : (a:Z)`a>0`->`a%a=0`.
+Lemma Z_mod_same : forall a:Z, (a > 0)%Z -> (a mod a)%Z = 0%Z.
 Proof.
-Intros a aPos.
-Generalize (Z_mod_plus `0` `1` a aPos).
-Replace `0+1*a` with `a`.
-Intros.
-Rewrite H.
-Compute.
-Trivial.
-Ring.
-Save.
+intros a aPos.
+generalize (Z_mod_plus 0 1 a aPos).
+replace (0 + 1 * a)%Z with a.
+intros.
+rewrite H.
+compute.
+trivial.
+ring.
+Qed.
 
-Lemma Z_div_same : (a:Z)`a>0`->`a/a=1`.
+Lemma Z_div_same : forall a:Z, (a > 0)%Z -> (a / a)%Z = 1%Z.
 Proof.
-Intros a aPos.
-Generalize (Z_div_plus `0` `1` a aPos).
-Replace `0+1*a` with `a`.
-Intros.
-Rewrite H.
-Compute.
-Trivial.
-Ring.
-Save.
+intros a aPos.
+generalize (Z_div_plus 0 1 a aPos).
+replace (0 + 1 * a)%Z with a.
+intros.
+rewrite H.
+compute.
+trivial.
+ring.
+Qed.
 
 (* some general lemmas for invariants *)
 
-Lemma iter_sqrt_pos: (x,z:Z)`x>0`->`z>0`->`(x/z+z)/2>0`.
+Lemma iter_sqrt_pos :
+ forall x z:Z, (x > 0)%Z -> (z > 0)%Z -> ((x / z + z) / 2 > 0)%Z.
 Proof.
-Intros x z xPos zPos.
-Assert `(x/z+z)>=2`.
-Assert `(x+z*z)>=z+z`.
-Assert `x+(z-1)*(z-1) >= 1`.
-Generalize (sqr_pos `z-1`).
-Intros.
-Omega.
-Replace `z*z` with `(z-1)*(z-1)+z+z-1`.
-Omega.
-Ring.
-Generalize (Z_div_ge `x+z*z` `z+z` `z` zPos H).
-Intro.
-Generalize (Z_div_plus x z z zPos).
-Intro H1.
-Rewrite H1 in H0.
-Clear H1.
-Generalize (Z_div_plus z `1` z zPos).
-Replace `1*z` with `z`.
-Intro H2.
-Rewrite H2 in H0.
-Clear H2.
-Generalize (Z_div_plus `0` `1` z zPos).
-Replace `1*z` with `z`.
-Replace `0+z` with `z`.
-Intro.
-Rewrite H1 in H0.
-Simpl in H0.
-Trivial.
-Trivial.
-Ring.
-Ring.
-Assert `2>0`.
-Omega.
-Generalize (Z_div_ge `x/z+z` `2` `2` H0 H).
-Replace `2/2` with `1`.
-Intro; Omega.
-Compute.
-Trivial.
-Save.
+intros x z xPos zPos.
+assert (x / z + z >= 2)%Z.
+assert (x + z * z >= z + z)%Z.
+assert (x + (z - 1) * (z - 1) >= 1)%Z.
+generalize (sqr_pos (z - 1)).
+intros.
+omega.
+replace (z * z)%Z with ((z - 1) * (z - 1) + z + z - 1)%Z.
+omega.
+ring.
+generalize (Z_div_ge (x + z * z) (z + z) z zPos H).
+intro.
+generalize (Z_div_plus x z z zPos).
+intro H1.
+rewrite H1 in H0.
+clear H1.
+generalize (Z_div_plus z 1 z zPos).
+replace (1 * z)%Z with z.
+intro H2.
+rewrite H2 in H0.
+clear H2.
+generalize (Z_div_plus 0 1 z zPos).
+replace (1 * z)%Z with z.
+replace (0 + z)%Z with z.
+intro.
+rewrite H1 in H0.
+simpl in H0.
+trivial.
+trivial.
+ring.
+ring.
+assert (2 > 0)%Z.
+omega.
+generalize (Z_div_ge (x / z + z) 2 2 H0 H).
+replace (2 / 2)%Z with 1%Z.
+intro; omega.
+compute.
+trivial.
+Qed.
 
-Lemma iter_sqrt_pos2 : (x:Z)`x>0`->`(x+1)/2>0`.
+Lemma iter_sqrt_pos2 : forall x:Z, (x > 0)%Z -> ((x + 1) / 2 > 0)%Z.
 Proof.
-Intros.
-Assert `x+1 >= 2`. Omega.
-Assert `(x+1)/2 >= 2/2`.
-Apply Z_div_ge; Try Omega.
-Assert `2/2 > 0`; Try Omega.
-Compute; Trivial.
-Save.
+intros.
+assert (x + 1 >= 2)%Z.
+ omega.
+assert ((x + 1) / 2 >= 2 / 2)%Z.
+apply Z_div_ge; try omega.
+assert (2 / 2 > 0)%Z; try omega.
+compute; trivial.
+Qed.
 
-Lemma iter_sqrt_invar1: (x,y,z:Z)
-  `x>0`->`y>0`->`z=(x/y+y)/2`->`2*y*z<=x+y*y`.
+Lemma iter_sqrt_invar1 :
+ forall x y z:Z,
+   (x > 0)%Z ->
+   (y > 0)%Z -> z = ((x / y + y) / 2)%Z -> (2 * y * z <= x + y * y)%Z.
 Proof.
-Intros x y z xPos yPos zVal.
-Assert `2*z <= x/y+y`.
-Rewrite zVal.
-Apply Z_mult_div_ge; Omega.
-Assert `2*y*z <= y*(x/y+y)`.
-Replace `2*y*z` with `y*(2*z)`; Try Ring.
-Apply Zle_Zmult_pos_left; Trivial Orelse Omega.
-Assert `y*(x/y+y) <= x+y*y`.
-Assert `y*(x/y+y) = y*(x/y)+y*y`; Try Ring. 
-Assert `y*(x/y) <= x`.
-Apply Z_mult_div_ge; Omega.
-Omega.
-Omega.
-Save.
+intros x y z xPos yPos zVal.
+assert (2 * z <= x / y + y)%Z.
+rewrite zVal.
+apply Z_mult_div_ge; omega.
+assert (2 * y * z <= y * (x / y + y))%Z.
+replace (2 * y * z)%Z with (y * (2 * z))%Z; try ring.
+apply Zle_Zmult_pos_left; trivial || omega.
+assert (y * (x / y + y) <= x + y * y)%Z.
+assert ((y * (x / y + y))%Z = (y * (x / y) + y * y)%Z); try ring.
+ assert (y * (x / y) <= x)%Z.
+apply Z_mult_div_ge; omega.
+omega.
+omega.
+Qed.
 
-Lemma iter_sqrt_invar2: (x,y,z:Z)
-  `x>0`->`y>0`->`z=(x/y+y)/2`->`2*y*(z+1)>x+y*y`.
+Lemma iter_sqrt_invar2 :
+ forall x y z:Z,
+   (x > 0)%Z ->
+   (y > 0)%Z ->
+   z = ((x / y + y) / 2)%Z -> (2 * y * (z + 1) > x + y * y)%Z.
 Proof.
-Intros x y z xPos yPos zVal.
-Assert TwoPos:`2>0`; Try Omega.
-Generalize (Z_div_mod_eq x y yPos).
-Generalize (Z_mod_lt x y yPos).
-Generalize (Z_div_mod_eq `x/y+y` `2` TwoPos).
-Generalize (Z_mod_lt `x/y+y` `2` TwoPos).
-Intros.
-Rewrite zVal.
-Replace `2*y*((x/y+y)/2+1)` with `y*(2*((x/y+y)/2))+y+y`; 
-  Try Ring.
-Replace `2*((x/y+y)/2)` with `x/y+y - (x/y+y)%2`.
-Replace `y*(x/y+y-(x/y+y)%2)` with `y*(x/y)+y*y-y*((x/y+y)%2)`.
-Replace `y*(x/y)` with `x - x%y`.
-Assert `y >= y*((x/y+y)%2)`.
-Pattern 1 y; Replace `y` with `y*1`.
-Apply Zge_Zmult_pos_left.
-Omega.
-Omega.
-Ring.
-Omega.
-Omega.
-Ring.
-Omega.
-Save.
+intros x y z xPos yPos zVal.
+assert TwoPos: (2 > 0)%Z; try omega.
+generalize (Z_div_mod_eq x y yPos).
+generalize (Z_mod_lt x y yPos).
+generalize (Z_div_mod_eq (x / y + y) 2 TwoPos).
+generalize (Z_mod_lt (x / y + y) 2 TwoPos).
+intros.
+rewrite zVal.
+replace (2 * y * ((x / y + y) / 2 + 1))%Z with
+ (y * (2 * ((x / y + y) / 2)) + y + y)%Z; try ring.
+replace (2 * ((x / y + y) / 2))%Z with
+ (x / y + y - (x / y + y) mod 2)%Z.
+replace (y * (x / y + y - (x / y + y) mod 2))%Z with
+ (y * (x / y) + y * y - y * ((x / y + y) mod 2))%Z.
+replace (y * (x / y))%Z with (x - x mod y)%Z.
+assert (y >= y * ((x / y + y) mod 2))%Z.
+pattern y 1; replace y with (y * 1)%Z.
+apply Zge_Zmult_pos_left.
+omega.
+omega.
+ring.
+omega.
+omega.
+ring.
+omega.
+Qed.
 
-Lemma iter_sqrt_invar3: (x,y,z:Z)
-`x>0` -> `y>0` -> `z=(x/y+y)/2` -> `x<(z+1)*(z+1)`.
+Lemma iter_sqrt_invar3 :
+ forall x y z:Z,
+   (x > 0)%Z ->
+   (y > 0)%Z -> z = ((x / y + y) / 2)%Z -> (x < (z + 1) * (z + 1))%Z.
 Proof.
-Intros x y z xPos yPos zVal.
-Cut `(z+1)*(z+1)-x > 0 `; Try Omega.
-Assert `(4*y*y)*((z+1)*(z+1)-x) >= 1`.
-Replace `(4*y*y)*((z+1)*(z+1)-x)` with
-  `(2*y*(z+1))*(2*y*(z+1)) - 4*y*y*x`; Try Ring.
-Generalize (iter_sqrt_invar2 x y z xPos yPos zVal).
-Intro.
-Assert `2*y*(z+1)*(2*y*(z+1)) > (x+y*y)*(x+y*y)`.
-Assert `2*y*(z+1)*(x+y*y) > (x+y*y)*(x+y*y)`.
-Apply Zgt_Zmult_right.
-Generalize (sqr_pos y).
-Omega.
-Assumption.
-Assert `2*y*(z+1)*(2*y*(z+1)) > 2*y*(z+1)*(x+y*y)`; Try Omega.
-Apply Zgt_Zmult_left; Try Assumption.
-Apply Zgt_ZERO_mult; Try Omega.
-Assert `z>=0`; Try Omega.
-Rewrite zVal.
-Apply Z_div_ge0; Try Omega.
-Assert `x/y>=0`; Try Omega.
-Apply Z_div_ge0; Try Omega.
-Assert `(x+y*y)*(x+y*y)-4*y*y*x >=0`; Try Omega.
-Replace `(x+y*y)*(x+y*y)-4*y*y*x` with `(x-y*y)*(x-y*y)`; Try Ring.
-Apply sqr_pos.
-Apply (Zmult_gt `4*y*y`).
-Apply Zgt_ZERO_mult; Try Omega.
-Omega.
-Save.
+intros x y z xPos yPos zVal.
+cut ((z + 1) * (z + 1) - x > 0)%Z; try omega.
+assert (4 * y * y * ((z + 1) * (z + 1) - x) >= 1)%Z.
+replace (4 * y * y * ((z + 1) * (z + 1) - x))%Z with
+ (2 * y * (z + 1) * (2 * y * (z + 1)) - 4 * y * y * x)%Z; try ring.
+generalize (iter_sqrt_invar2 x y z xPos yPos zVal).
+intro.
+assert
+ (2 * y * (z + 1) * (2 * y * (z + 1)) > (x + y * y) * (x + y * y))%Z.
+assert (2 * y * (z + 1) * (x + y * y) > (x + y * y) * (x + y * y))%Z.
+apply Zgt_Zmult_right.
+generalize (sqr_pos y).
+omega.
+assumption.
+assert
+ (2 * y * (z + 1) * (2 * y * (z + 1)) > 2 * y * (z + 1) * (x + y * y))%Z;
+ try omega.
+apply Zgt_Zmult_left; try assumption.
+apply Zgt_ZERO_mult; try omega.
+assert (z >= 0)%Z; try omega.
+rewrite zVal.
+apply Z_div_ge0; try omega.
+assert (x / y >= 0)%Z; try omega.
+apply Z_div_ge0; try omega.
+assert ((x + y * y) * (x + y * y) - 4 * y * y * x >= 0)%Z; try omega.
+replace ((x + y * y) * (x + y * y) - 4 * y * y * x)%Z with
+ ((x - y * y) * (x - y * y))%Z; try ring.
+apply sqr_pos.
+apply (Zmult_gt (4 * y * y)).
+apply Zgt_ZERO_mult; try omega.
+omega.
+Qed.
 
 
 
 
-Lemma iter_sqrt_invar4: (x,y,z:Z)
-`x>0` -> `y>0` -> `z=(x/y+y)/2` -> `z>=y` -> `y*y<= x`.
+Lemma iter_sqrt_invar4 :
+ forall x y z:Z,
+   (x > 0)%Z ->
+   (y > 0)%Z -> z = ((x / y + y) / 2)%Z -> (z >= y)%Z -> (y * y <= x)%Z.
 Proof.
-Intros x y z xPos yPos zVal zGey.
-Generalize (iter_sqrt_invar1 x y z xPos yPos zVal); Intros.
-Assert `y*y <= y*z`.
-Apply Zle_Zmult_pos_left; Try Omega.
-Assert `2*y*z = y*z+y*z`; Try Ring.
-Omega.
-Save.
+intros x y z xPos yPos zVal zGey.
+generalize (iter_sqrt_invar1 x y z xPos yPos zVal); intros.
+assert (y * y <= y * z)%Z.
+apply Zle_Zmult_pos_left; try omega.
+assert ((2 * y * z)%Z = (y * z + y * z)%Z); try ring.
+omega.
+Qed.
 
 
 
 
 (* beginning of proof obligations *)
 
-(* Why obligation from file "sqrt.mlw", characters 391-392 *)
-Lemma sqrt_po_1 : 
-  (x: Z)
-  (Pre7: `x >= 0`)
-  (Test6: `x = 0`)
-  `0 * 0 <= x` /\ `x < (0 + 1) * (0 + 1)`.
-Proof. (* sqrt_po_1 *)
-Auto with *.
-Save.
-
-(* Why obligation from file "sqrt.mlw", characters 417-418 *)
-Lemma sqrt_po_2 : 
-  (x: Z)
-  (Pre7: `x >= 0`)
-  (Test5: `x <> 0`)
-  (Test4: `x <= 3`)
-  `1 * 1 <= x` /\ `x < (1 + 1) * (1 + 1)`.
-Proof. (* sqrt_po_2 *)
-Auto with *.
-Save.
-
-(* Why obligation from file "sqrt.mlw", characters 460-467 *)
-Lemma sqrt_po_3 : 
-  (x: Z)
-  (Pre7: `x >= 0`)
-  (Test5: `x <> 0`)
-  (Test3: `x > 3`)
-  (y: Z)
-  (Post5: y = x)
-  ~(`2` = `0`).
-Proof. (* sqrt_po_3 *)
-Auto with *.
-Save.
-
-(* Why obligation from file "sqrt.mlw", characters 654-660 *)
-Lemma sqrt_po_4 : 
-  (x: Z)
-  (Pre7: `x >= 0`)
-  (Test5: `x <> 0`)
-  (Test3: `x > 3`)
-  (y: Z)
-  (Post5: y = x)
-  (Pre6: ~(`2` = `0`))
-  (z: Z)
-  (Post4: z = (Zdiv (`x + 1`) `2`))
-  (Variant1: Z)
-  (y1: Z)
-  (z1: Z)
-  (Pre5: Variant1 = y1)
-  (Pre4: `z1 > 0` /\ `y1 > 0` /\ `z1 = (Zdiv ((Zdiv x y1) + y1) 2)` /\
-         `x < (y1 + 1) * (y1 + 1)` /\ `x < (z1 + 1) * (z1 + 1)`)
-  (Test2: `z1 < y1`)
-  (y2: Z)
-  (Post1: y2 = z1)
-  (Pre2: ~(`2` = `0`))
-  ~(z1 = `0`).
-Proof. 
-Intuition.
-Save.
-
-
-(* Why obligation from file "sqrt.mlw", characters 636-670 *)
-Lemma sqrt_po_5 : 
-  (x: Z)
-  (Pre7: `x >= 0`)
-  (Test5: `x <> 0`)
-  (Test3: `x > 3`)
-  (y: Z)
-  (Post5: y = x)
-  (Pre6: ~(`2` = `0`))
-  (z: Z)
-  (Post4: z = (Zdiv (`x + 1`) `2`))
-  (Variant1: Z)
-  (y1: Z)
-  (z1: Z)
-  (Pre5: Variant1 = y1)
-  (Pre4: `z1 > 0` /\ `y1 > 0` /\ `z1 = (Zdiv ((Zdiv x y1) + y1) 2)` /\
-         `x < (y1 + 1) * (y1 + 1)` /\ `x < (z1 + 1) * (z1 + 1)`)
-  (Test2: `z1 < y1`)
-  (y2: Z)
-  (Post1: y2 = z1)
-  (Pre2: ~(`2` = `0`))
-  (Pre3: ~(z1 = `0`))
-  (z2: Z)
-  (Post2: z2 = (Zdiv (`(Zdiv x z1) + z1`) `2`))
-  (`z2 > 0` /\ `y2 > 0` /\ `z2 = (Zdiv ((Zdiv x y2) + y2) 2)` /\
-  `x < (y2 + 1) * (y2 + 1)` /\ `x < (z2 + 1) * (z2 + 1)`) /\ (Zwf `0` y2 y1).
-Proof. 
-Unfold Zwf; Intuition.
-Subst z2.
-Apply iter_sqrt_pos; Omega.
-Subst y2; Assumption.
-Subst y2; Assumption.
-Apply (iter_sqrt_invar3 x z1); Auto.
-Omega.
-Save.
-
-(* Why obligation from file "sqrt.mlw", characters 525-613 *)
-Lemma sqrt_po_6 : 
-  (x: Z)
-  (Pre7: `x >= 0`)
-  (Test5: `x <> 0`)
-  (Test3: `x > 3`)
-  (y: Z)
-  (Post5: y = x)
-  (Pre6: ~(`2` = `0`))
-  (z: Z)
-  (Post4: z = (Zdiv (`x + 1`) `2`))
-  `z > 0` /\ `y > 0` /\ `z = (Zdiv ((Zdiv x y) + y) 2)` /\
-  `x < (y + 1) * (y + 1)` /\ `x < (z + 1) * (z + 1)`.
-Proof. 
-(* sqrt_po_6 *)
-Intuition.
-Subst z.
-Assert `(x+1)/2 >= 1`.
-Pattern 2 `1`; Replace `1` with `2/2`; Trivial.
-Apply Z_div_ge; Try Omega.
-Omega.
-Subst y.
-Assert `x/x+x = x+1`.
-Assert xPos:`x>0`; Try Omega.
-Generalize (Z_div_same x xPos). 
-Intro.
-Rewrite H; Omega.
-Rewrite H; Trivial.
-
-Subst y.
-Assert `(x+1)*(x+1) >= (x+1)*1`.
-Apply Zge_Zmult_pos_left; Try Omega.
-Assert `(x+1)*1 = x+1`; Try Ring.
-Omega.
-
-Subst z.
-Apply (iter_sqrt_invar3 x x); Try Omega.
-Assert `x/x+x = x+1`.
-Assert xPos:`x>0`; Try Omega.
-Generalize (Z_div_same x xPos). 
-Intro.
-Rewrite H; Omega.
-Rewrite H; Trivial.
-Save.
-
-(* Why obligation from file "sqrt.mlw", characters 679-681 *)
-Lemma sqrt_po_7 : 
-  (x: Z)
-  (Pre7: `x >= 0`)
-  (Test5: `x <> 0`)
-  (Test3: `x > 3`)
-  (y: Z)
-  (Post5: y = x)
-  (Pre6: ~(`2` = `0`))
-  (z: Z)
-  (Post4: z = (Zdiv (`x + 1`) `2`))
-  (y1: Z)
-  (z1: Z)
-  (Post3: (`z1 > 0` /\ `y1 > 0` /\ `z1 = (Zdiv ((Zdiv x y1) + y1) 2)` /\
-          `x < (y1 + 1) * (y1 + 1)` /\ `x < (z1 + 1) * (z1 + 1)`) /\
-          `z1 >= y1`)
-  `y1 * y1 <= x` /\ `x < (y1 + 1) * (y1 + 1)`.
+(* Why obligation from file , characters 391-392 *)
+Lemma sqrt_po_1 :
+ forall (x:Z) (Pre7:(x >= 0)%Z) (Test6:x = 0%Z),
+   (0 * 0 <= x)%Z /\ (x < (0 + 1) * (0 + 1))%Z.
+ (* sqrt_po_1 *)
 Proof.
-Intuition.
-Apply (iter_sqrt_invar4 x y1 z1); Try Omega.
-Save.
+auto with *.
+Qed.
+
+(* Why obligation from file , characters 417-418 *)
+Lemma sqrt_po_2 :
+ forall (x:Z) (Pre7:(x >= 0)%Z) (Test5:x <> 0%Z) (Test4:(x <= 3)%Z),
+   (1 * 1 <= x)%Z /\ (x < (1 + 1) * (1 + 1))%Z.
+ (* sqrt_po_2 *)
+Proof.
+auto with *.
+Qed.
+
+(* Why obligation from file , characters 460-467 *)
+Lemma sqrt_po_3 :
+ forall (x:Z) (Pre7:(x >= 0)%Z) (Test5:x <> 0%Z) (Test3:(x > 3)%Z)
+   (y:Z) (Post5:y = x), 2%Z <> 0%Z.
+ (* sqrt_po_3 *)
+Proof.
+auto with *.
+Qed.
+
+(* Why obligation from file , characters 654-660 *)
+Lemma sqrt_po_4 :
+ forall (x:Z) (Pre7:(x >= 0)%Z) (Test5:x <> 0%Z) (Test3:(x > 3)%Z)
+   (y:Z) (Post5:y = x) (Pre6:2%Z <> 0%Z) (z:Z)
+   (Post4:z = ((x + 1) / 2)%Z) (Variant1 y1 z1:Z) (Pre5:Variant1 = y1)
+   (Pre4:(z1 > 0)%Z /\
+         (y1 > 0)%Z /\
+         z1 = ((x / y1 + y1) / 2)%Z /\
+         (x < (y1 + 1) * (y1 + 1))%Z /\ (x < (z1 + 1) * (z1 + 1))%Z)
+   (Test2:(z1 < y1)%Z) (y2:Z) (Post1:y2 = z1) (Pre2:2%Z <> 0%Z),
+   z1 <> 0%Z.
+ Proof.
+ intuition.
+Qed.
+
+
+(* Why obligation from file , characters 636-670 *)
+Lemma sqrt_po_5 :
+ forall (x:Z) (Pre7:(x >= 0)%Z) (Test5:x <> 0%Z) (Test3:(x > 3)%Z)
+   (y:Z) (Post5:y = x) (Pre6:2%Z <> 0%Z) (z:Z)
+   (Post4:z = ((x + 1) / 2)%Z) (Variant1 y1 z1:Z) (Pre5:Variant1 = y1)
+   (Pre4:(z1 > 0)%Z /\
+         (y1 > 0)%Z /\
+         z1 = ((x / y1 + y1) / 2)%Z /\
+         (x < (y1 + 1) * (y1 + 1))%Z /\ (x < (z1 + 1) * (z1 + 1))%Z)
+   (Test2:(z1 < y1)%Z) (y2:Z) (Post1:y2 = z1) (Pre2:2%Z <> 0%Z)
+   (Pre3:z1 <> 0%Z) (z2:Z) (Post2:z2 = ((x / z1 + z1) / 2)%Z),
+   ((z2 > 0)%Z /\
+    (y2 > 0)%Z /\
+    z2 = ((x / y2 + y2) / 2)%Z /\
+    (x < (y2 + 1) * (y2 + 1))%Z /\ (x < (z2 + 1) * (z2 + 1))%Z) /\
+   Zwf 0 y2 y1.
+ Proof.
+ unfold Zwf; intuition.
+subst z2.
+apply iter_sqrt_pos; omega.
+subst y2; assumption.
+subst y2; assumption.
+apply (iter_sqrt_invar3 x z1); auto.
+omega.
+Qed.
+
+(* Why obligation from file , characters 525-613 *)
+Lemma sqrt_po_6 :
+ forall (x:Z) (Pre7:(x >= 0)%Z) (Test5:x <> 0%Z) (Test3:(x > 3)%Z)
+   (y:Z) (Post5:y = x) (Pre6:2%Z <> 0%Z) (z:Z)
+   (Post4:z = ((x + 1) / 2)%Z),
+   (z > 0)%Z /\
+   (y > 0)%Z /\
+   z = ((x / y + y) / 2)%Z /\
+   (x < (y + 1) * (y + 1))%Z /\ (x < (z + 1) * (z + 1))%Z.
+ (* sqrt_po_6 *)
+Proof.
+intuition.
+subst z.
+assert ((x + 1) / 2 >= 1)%Z.
+pattern 1%Z 2; replace 1%Z with (2 / 2)%Z; trivial.
+apply Z_div_ge; try omega.
+omega.
+subst y.
+assert ((x / x + x)%Z = (x + 1)%Z).
+assert xPos: (x > 0)%Z; try omega.
+generalize (Z_div_same x xPos).
+ intro.
+rewrite H; omega.
+rewrite H; trivial.
+
+subst y.
+assert ((x + 1) * (x + 1) >= (x + 1) * 1)%Z.
+apply Zge_Zmult_pos_left; try omega.
+assert (((x + 1) * 1)%Z = (x + 1)%Z); try ring.
+omega.
+
+subst z.
+apply (iter_sqrt_invar3 x x); try omega.
+assert ((x / x + x)%Z = (x + 1)%Z).
+assert xPos: (x > 0)%Z; try omega.
+generalize (Z_div_same x xPos).
+ intro.
+rewrite H; omega.
+rewrite H; trivial.
+Qed.
+
+(* Why obligation from file , characters 679-681 *)
+Lemma sqrt_po_7 :
+ forall (x:Z) (Pre7:(x >= 0)%Z) (Test5:x <> 0%Z) (Test3:(x > 3)%Z)
+   (y:Z) (Post5:y = x) (Pre6:2%Z <> 0%Z) (z:Z)
+   (Post4:z = ((x + 1) / 2)%Z) (y1 z1:Z)
+   (Post3:((z1 > 0)%Z /\
+           (y1 > 0)%Z /\
+           z1 = ((x / y1 + y1) / 2)%Z /\
+           (x < (y1 + 1) * (y1 + 1))%Z /\ (x < (z1 + 1) * (z1 + 1))%Z) /\
+          (z1 >= y1)%Z),
+   (y1 * y1 <= x)%Z /\ (x < (y1 + 1) * (y1 + 1))%Z.
+Proof.
+intuition.
+apply (iter_sqrt_invar4 x y1 z1); try omega.
+Qed.
 
